src/Lustre/Normalization/LNormalization.v
@@ -1,24 +1,28 @@
 From Velus Require Import Common Ident.
 From Velus Require Import Operators Environment.
 From Velus Require Import CoindStreams.
-From Velus Require Import Lustre.LSyntax Lustre.LOrdered Lustre.LTyping Lustre.LClocking Lustre.LSemantics.
+From Velus Require Import Lustre.LSyntax Lustre.LTyping Lustre.LClocking.
+From Velus Require Import Lustre.LCausality Lustre.LOrdered.
+From Velus Require Import Lustre.LSemantics LClockSemantics.
 From Velus Require Import Lustre.Normalization.Normalization.
 From Velus Require Import Lustre.Normalization.Correctness.
 From Velus Require Import Lustre.Normalization.Idempotence.
 
 Local Set Warnings "-masking-absolute-name".
 Module Type LNORMALIZATION
-       (Import Ids : IDS)
-       (Import Op : OPERATORS)
-       (Import OpAux : OPERATORS_AUX Op)
-       (Import Str : COINDSTREAMS Op OpAux)
-       (Import Syn : LSYNTAX Ids Op)
-       (Import Typ : LTYPING Ids Op Syn)
-       (Import Clo : LCLOCKING Ids Op Syn)
-       (Import Lord : LORDERED Ids Op Syn)
-       (Import Sem : LSEMANTICS Ids Op OpAux Syn Lord Str).
+       (Ids : IDS)
+       (Op : OPERATORS)
+       (OpAux : OPERATORS_AUX Op)
+       (Str : COINDSTREAMS Op OpAux)
+       (Syn : LSYNTAX Ids Op)
+       (Typ : LTYPING Ids Op Syn)
+       (Clo : LCLOCKING Ids Op Syn)
+       (Cau : LCAUSALITY Ids Op Syn)
+       (Ord : LORDERED Ids Op Syn)
+       (Sem : LSEMANTICS Ids Op OpAux Syn Ord Str)
+       (ClSem : LCLOCKSEMANTICS Ids Op OpAux Syn Typ Clo Cau Ord Str Sem).
   Declare Module Norm : NORMALIZATION Ids Op OpAux Syn.
-  (* Declare Module Export Correct : CORRECTNESS Ids Op OpAux Str Syn Typ Clo Lord Sem Norm. *)
+  Declare Module Export Correct : CORRECTNESS Ids Op OpAux Str Syn Typ Clo Cau Ord Sem ClSem Norm.
   Declare Module Idempotence : IDEMPOTENCE Ids Op OpAux Syn Norm.
 End LNORMALIZATION.
 
@@ -30,10 +34,12 @@ Module LNormalizationFun
        (Syn : LSYNTAX Ids Op)
        (Typ : LTYPING Ids Op Syn)
        (Clo : LCLOCKING Ids Op Syn)
-       (Lord : LORDERED Ids Op Syn)
-       (Sem : LSEMANTICS Ids Op OpAux Syn Lord Str)
-       <: LNORMALIZATION Ids Op OpAux Str Syn Typ Clo Lord Sem.
+       (Cau : LCAUSALITY Ids Op Syn)
+       (Ord : LORDERED Ids Op Syn)
+       (Sem : LSEMANTICS Ids Op OpAux Syn Ord Str)
+       (ClSem : LCLOCKSEMANTICS Ids Op OpAux Syn Typ Clo Cau Ord Str Sem)
+       <: LNORMALIZATION Ids Op OpAux Str Syn Typ Clo Cau Ord Sem ClSem.
   Module Norm := NormalizationFun Ids Op OpAux Syn.
-  (* Module Export Correct := CorrectnessFun Ids Op OpAux Str Syn Typ Clo Lord Sem Norm. *)
+  Module Export Correct := CorrectnessFun Ids Op OpAux Str Syn Typ Clo Cau Ord Sem ClSem Norm.
   Module Idempotence := IdempotenceFun Ids Op OpAux Syn Norm.
 End LNormalizationFun.
