src/Lustre/Normalization/NCausality.v
@@ -1,0 +1,2002 @@
+From Coq Require Import List.
+Import List.ListNotations.
+Open Scope list_scope.
+From Coq Require Import Permutation.
+From Coq Require Import Decidable.
+From Coq Require Import Omega.
+From Coq Require Import Setoid Morphisms.
+
+From Velus Require Import Common Ident Clocks.
+From Velus Require Import Operators Environment.
+From Velus Require Import Lustre.LSyntax Lustre.LClocking Lustre.LCausality.
+From Velus Require Import Lustre.Normalization.Fresh Lustre.Normalization.Normalization.
+
+(** * Conservation of causality through normalization *)
+
+Local Set Warnings "-masking-absolute-name".
+Module Type NCAUSALITY
+       (Import Ids : IDS)
+       (Op : OPERATORS)
+       (OpAux : OPERATORS_AUX Op)
+       (Import Syn : LSYNTAX Ids Op)
+       (Import Clo : LCLOCKING Ids Op Syn)
+       (Import Cau : LCAUSALITY Ids Op Syn)
+       (Import Norm : NORMALIZATION Ids Op OpAux Syn).
+
+  Import Fresh Tactics.
+
+  (** Some auxiliary stuff *)
+
+  Fact in_vars_defined_concat : forall x eqs eqs',
+      In eqs eqs' ->
+      In x (vars_defined eqs) ->
+      In x (vars_defined (concat eqs')).
+  Proof.
+    intros * Hin1 Hin2.
+    unfold vars_defined in *. rewrite flat_map_concat_map in *.
+    apply in_concat in Hin2 as [xs [Hin2 Hin3]].
+    apply in_map_iff in Hin3 as [[xs' es] [? Hin3]]; simpl in *; subst.
+    eapply incl_concat_map with (x0:=(xs, es)); simpl; auto.
+    eapply in_concat'; eauto.
+  Qed.
+
+  Fact vars_defined_combine : forall xs es,
+      length xs = length es ->
+      vars_defined (combine xs es) = concat xs.
+  Proof.
+    intros * Hlen.
+    unfold vars_defined. rewrite flat_map_concat_map, combine_map_fst'; auto.
+  Qed.
+
+  (** If an expression is wc with regards to an environment, all it's
+      left-free vars appear in the environment *)
+
+  Hint Resolve In_InMembers.
+  Fact wc_exp_Is_free_left : forall G vars x e,
+      wc_exp G vars e ->
+      Is_free_left x e ->
+      InMembers x vars.
+  Proof with eauto.
+    induction e using exp_ind2; intros Hwc Hfree;
+      inv Hwc; inv Hfree...
+    Local Ltac Forall_Exists_free H :=
+      eapply Forall_Exists, Exists_exists in H as [? [_ [H ?]]]; eauto;
+      simpl in H; destruct H as [? ?]; eauto.
+    - (* binop *) destruct H0; eauto.
+    - (* fby *)
+      eapply Forall_Forall in H; eauto. clear H4.
+      Forall_Exists_free H2.
+    - (* when *)
+      destruct H1 as [?|Hfree]; subst...
+      eapply Forall_Forall in H; eauto. clear H4.
+      Forall_Exists_free Hfree.
+    - (* merge *)
+      destruct H2 as [?|Hfree]; subst...
+      eapply Forall_Forall in H; eauto. clear H5.
+      eapply Forall_Forall in H0; eauto. clear H6.
+      destruct Hfree as [Hfree|Hfree]; Forall_Exists_free Hfree.
+    - (* ite *)
+      eapply Forall_Forall in H; eauto. clear H6.
+      eapply Forall_Forall in H0; eauto. clear H7.
+      destruct H2 as [Hfree|[Hfree|Hfree]]; eauto; Forall_Exists_free Hfree.
+    - (* app *)
+      eapply Forall_Forall in H0; eauto. clear H5.
+      Forall_Exists_free H2.
+    - (* app (reset) *)
+      eapply Forall_Forall in H0; eauto. clear H5.
+      inv H2...
+      Forall_Exists_free H3.
+  Qed.
+
+  (** A clocking + causality property : *)
+
+  Inductive Is_free_left_ck (x : ident) : exp -> Prop :=
+  | IFLvar : forall y ty ck name,
+      x = y \/
+      Is_free_in_clock x ck ->
+      Is_free_left_ck x (Evar y (ty, (ck, name)))
+  | IFLunop : forall op e ty ck name,
+      Is_free_left_ck x e \/
+      Is_free_in_clock x ck ->
+      Is_free_left_ck x (Eunop op e (ty, (ck, name)))
+  | IFLbinop : forall op e1 e2 ty ck name,
+      Is_free_left_ck x e1 \/
+      Is_free_left_ck x e2 \/
+      Is_free_in_clock x ck ->
+      Is_free_left_ck x (Ebinop op e1 e2 (ty, (ck, name)))
+  | IFLfby : forall e0s es a,
+      Exists (Is_free_left_ck x) e0s \/
+      Exists (Is_free_in_clock x) (map clock_of_nclock a) ->
+      Is_free_left_ck x (Efby e0s es a)
+  | IFLwhen : forall es y b tys ck name,
+      x = y \/
+      Exists (Is_free_left_ck x) es \/
+      Is_free_in_clock x ck ->
+      Is_free_left_ck x (Ewhen es y b (tys, (ck, name)))
+  | IFLmerge : forall ets efs y tys ck name,
+      x = y \/
+      Exists (Is_free_left_ck x) ets \/
+      Exists (Is_free_left_ck x) efs \/
+      Is_free_in_clock x ck ->
+      Is_free_left_ck x (Emerge y ets efs (tys, (ck, name)))
+  | IFLite : forall e ets efs tys ck name,
+      Is_free_left_ck x e \/
+      Exists (Is_free_left_ck x) ets \/
+      Exists (Is_free_left_ck x) efs \/
+      Is_free_in_clock x ck ->
+      Is_free_left_ck x (Eite e ets efs (tys, (ck, name)))
+  | IFLapp : forall f es a,
+      Exists (Is_free_left_ck x) es ->
+      Is_free_left_ck x (Eapp f es None a)
+  | IFLreset : forall f es r a,
+      Exists (Is_free_left_ck x) (r :: es) ->
+      Is_free_left_ck x (Eapp f es (Some r) a).
+  Hint Constructors Is_free_left_ck.
+
+  Inductive Is_causal_ck (inputs : list ident) : list equation -> Prop :=
+  | ICnil:
+      Is_causal_ck inputs []
+  | ICcons: forall eq eqs,
+      Is_causal_ck inputs eqs ->
+      (forall x, Exists (Is_free_left_ck x) (snd eq) ->
+            In x (vars_defined eqs) \/ In x inputs) ->
+      Is_causal_ck inputs (eq :: eqs).
+  Hint Constructors Is_causal_ck.
+
+  Fact Is_free_left_Is_free_left_ck : forall x e,
+      Is_free_left x e ->
+      Is_free_left_ck x e.
+  Proof.
+    induction e using exp_ind2; intros Hfree; inv Hfree;
+      try (destruct a as (ty&ck&name)); auto.
+    - (* binop *)
+      destruct H0; auto.
+    - (* fby *)
+      eapply Forall_Exists in H2; eauto.
+      constructor. left.
+      eapply Exists_Exists; [|eauto]. intros ? [? ?]; eauto.
+    - (* when *)
+      destruct H1; auto.
+      eapply Forall_Exists in H; eauto.
+      constructor. right; left.
+      eapply Exists_Exists; [|eauto]. intros ? [? ?]; eauto.
+    - (* merge *)
+      destruct H2 as [?|[?|?]]; auto.
+      + eapply Forall_Exists in H; eauto.
+        constructor. right; left.
+        eapply Exists_Exists; [|eauto]. intros ? [? ?]; eauto.
+      + eapply Forall_Exists in H0; eauto.
+        constructor. right; right; left.
+        eapply Exists_Exists; [|eauto]. intros ? [? ?]; eauto.
+    - (* ite *)
+      destruct H2 as [?|[?|?]]; auto.
+      + eapply Forall_Exists in H; eauto.
+        constructor. right; left.
+        eapply Exists_Exists; [|eauto]. intros ? [? ?]; eauto.
+      + eapply Forall_Exists in H0; eauto.
+        constructor. right; right; left.
+        eapply Exists_Exists; [|eauto]. intros ? [? ?]; eauto.
+    - (* app *)
+      eapply Forall_Exists in H0; eauto.
+      constructor.
+      eapply Exists_Exists; [|eauto]. intros ? [? ?]; eauto.
+    - (* app (reset) *)
+      inv H2; auto.
+      eapply Forall_Exists in H0; eauto.
+      constructor.
+      eapply Exists_Exists; [|eauto]. intros ? [? ?]; eauto.
+  Qed.
+
+  Fact Is_causal_ck_Is_causal : forall inputs eqs,
+      Is_causal_ck inputs eqs ->
+      Is_causal inputs eqs.
+  Proof.
+    intros * Hcaus. induction Hcaus; auto.
+    constructor; auto.
+    intros ? Hfree. eapply H.
+    eapply Exists_Exists; [|eauto].
+    intros. eapply Is_free_left_Is_free_left_ck; eauto.
+  Qed.
+
+  Fact Exists_clocksof : forall x es,
+      Exists (Is_free_in_clock x) (clocksof es) <->
+      Exists (fun e => Exists (Is_free_in_clock x) (clockof e)) es.
+  Proof.
+    intros *.
+    unfold clocksof. rewrite flat_map_concat_map, Exists_concat, Exists_map. reflexivity.
+  Qed.
+
+  Hint Constructors Is_free_left.
+
+  Lemma wc_normalized_lexp_clockof_free_in : forall G vars e,
+      normalized_lexp e ->
+      wc_exp G vars e ->
+      forall x, Exists (Is_free_in_clock x) (clockof e) ->
+           Is_free_left x e \/
+           exists y, exists ck', Is_free_left y e /\ In (y, ck') vars /\ Is_free_in_clock x ck'.
+  Proof.
+    intros * Hnormed Hwc ? Hex; induction Hnormed; inv Hwc;
+      simpl in Hex; apply Exists_singl in Hex.
+    - (* const *) inv Hex.
+    - (* var *)
+      right. exists x0. exists ck.
+      repeat split; auto.
+    - (* var *)
+      right. exists x0. exists ck.
+      repeat split; auto.
+    - (* unop *)
+      rewrite H4 in IHHnormed.
+      specialize (IHHnormed H1 (Exists_cons_hd _ _ _ Hex)) as [IHe|[y [ck' [?[? ?]]]]]; auto.
+      right. exists y. exists ck'. repeat split; auto.
+    - (* binop *)
+      rewrite H6 in IHHnormed1.
+      specialize (IHHnormed1 H3 (Exists_cons_hd _ _ _ Hex)) as [IHe1|[y [ck' [Hfree [Hin Hex']]]]]; auto.
+      right. exists y. exists ck'. repeat split; auto.
+     - (* when *)
+      simpl in *; rewrite app_nil_r in *.
+      inv Hex; auto.
+      symmetry in H7; singleton_length.
+      apply Forall_singl in H3. apply Forall_singl in H6; subst.
+      specialize (IHHnormed H3 (Exists_cons_hd _ _ _ H1)) as [Hex|[y [ck' [Hfree [Hin Hex]]]]]; auto.
+      right. exists y. exists ck'. repeat split; auto.
+  Qed.
+
+  Corollary wc_normalized_lexps_clocksof_free_in : forall G vars es,
+      Forall normalized_lexp es ->
+      Forall (wc_exp G vars) es ->
+      forall x, Exists (Is_free_in_clock x) (clocksof es) ->
+           Exists (fun e => Is_free_left x e \/
+                         exists y, exists ck', Is_free_left y e /\ In (y, ck') vars /\ Is_free_in_clock x ck') es.
+  Proof.
+    intros * Hnorm Hwc x Hex.
+    unfold clocksof in Hex. rewrite flat_map_concat_map, Exists_concat, Exists_map in Hex.
+    rewrite Exists_exists in *. destruct Hex as [e [Hin Hex]].
+    exists e. split; auto.
+    eapply wc_normalized_lexp_clockof_free_in; eauto.
+    1,2:eapply Forall_forall in Hin; eauto.
+  Qed.
+
+  Lemma wc_normalized_lexp_Is_free_left : forall G vars e,
+      normalized_lexp e ->
+      wc_exp G vars e ->
+      forall x, Is_free_left_ck x e ->
+           Is_free_left x e \/
+           exists y, exists ck', Is_free_left y e /\ In (y, ck') vars /\ Is_free_in_clock x ck'.
+  Proof.
+    intros * Hnormed Hwc ? Hex; induction Hnormed; inv Hwc; inv Hex.
+    - (* var *)
+      destruct H1; subst; eauto 10.
+    - (* var *)
+      destruct H1; subst; eauto 10.
+    - (* unop *)
+      destruct H0.
+      + eapply IHHnormed in H as [?|[y [ck' [? [? ?]]]]]; eauto 10.
+      + eapply wc_normalized_lexp_clockof_free_in in Hnormed as [?|[y [ck' [? [? ?]]]]]; eauto 10.
+        rewrite H4; auto.
+    - (* binop *)
+      destruct H0 as [?|[?|?]].
+      + eapply IHHnormed1 in H as [?|[y [ck' [? [? ?]]]]]; eauto 10.
+      + eapply IHHnormed2 in H as [?|[y [ck' [? [? ?]]]]]; eauto 10.
+      + eapply wc_normalized_lexp_clockof_free_in in Hnormed1 as [?|[y [ck' [? [? ?]]]]]; eauto 10.
+        rewrite H6; auto.
+     - (* when *)
+       apply Forall_singl in H3.
+       destruct H0 as [?|[Hex|Hex]]; auto.
+       + apply Exists_singl in Hex. eapply IHHnormed in Hex as [?|[y [ck' [? [? ?]]]]]; eauto 10.
+       + simpl in H7. symmetry in H7. rewrite app_nil_r in H7. singleton_length.
+         apply Forall_singl in H6; subst. inv Hex; auto.
+         eapply wc_normalized_lexp_clockof_free_in in Hnormed as [?|[y [ck' [? [? ?]]]]]; eauto.
+         2:rewrite Hsingl; auto.
+         right. exists y. exists ck'. repeat split; auto.
+  Qed.
+
+  Corollary wc_normalized_lexps_Is_free_left : forall G vars es,
+      Forall normalized_lexp es ->
+      Forall (wc_exp G vars) es ->
+      forall x, Exists (Is_free_left_ck x) es ->
+           Exists (fun e => Is_free_left x e \/
+                         exists y, exists ck', Is_free_left y e /\ In (y, ck') vars /\ Is_free_in_clock x ck') es.
+  Proof.
+    intros * Hnorm Hwc x Hex.
+    simpl_forall.
+    eapply Forall_Exists in Hex; eauto. clear Hnorm.
+    eapply Exists_Exists; [|eauto].
+    intros ? [[? ?] ?].
+    eapply wc_normalized_lexp_Is_free_left; eauto.
+  Qed.
+
+  Lemma wc_normalized_cexp_clockof_free_in : forall G vars e,
+      normalized_cexp e ->
+      wc_exp G vars e ->
+      forall x, Exists (Is_free_in_clock x) (clockof e) ->
+           Is_free_left x e \/
+           exists y, exists ck', Is_free_left y e /\ In (y, ck') vars /\ Is_free_in_clock x ck'.
+  Proof.
+    intros * Hnormed Hwc ? Hex; induction Hnormed;
+      simpl in Hex; try apply Exists_singl in Hex.
+    - (* merge *)
+      inv Hwc; simpl in *; rewrite app_nil_r in *.
+      clear IHHnormed2 H5 H8 H10.
+      symmetry in H9; singleton_length.
+      apply Forall_singl in H4. apply Forall_singl in H7; subst.
+      assert (Is_free_in_clock x (Con ck x0 true)) as Hfree by (right; auto).
+      specialize (IHHnormed1 H4 (Exists_cons_hd _ _ _ Hfree)) as [Hex'|[y [ck' [Hfree' [Hin Hex']]]]].
+      + left; auto.
+      + right. exists y. exists ck'. repeat split; auto.
+    - (* ite *)
+      inv Hwc.
+      eapply wc_normalized_lexp_clockof_free_in in H as [Hex'|[y [ck' [Hfree' [Hin Hex']]]]]; eauto.
+      2: rewrite H8; eauto.
+      right. exists y. exists ck'. repeat split; eauto.
+    - (* lexp *)
+      eapply wc_normalized_lexp_clockof_free_in in Hex; eauto.
+  Qed.
+
+  Lemma wc_normalized_cexp_Is_free_left : forall G vars e,
+      normalized_cexp e ->
+      wc_exp G vars e ->
+      forall x, Is_free_left_ck x e ->
+           Is_free_left x e \/
+           exists y, exists ck', Is_free_left y e /\ In (y, ck') vars /\ Is_free_in_clock x ck'.
+  Proof.
+    intros * Hnormed Hwc ? Hex; induction Hnormed.
+    1,2:inv Hwc; inv Hex.
+    - (* merge *)
+      apply Forall_singl in H4. apply Forall_singl in H5.
+      simpl in *. symmetry in H9, H10. rewrite app_nil_r in H9, H10.
+      repeat singleton_length.
+      apply Forall_singl in H7; apply Forall_singl in H8; subst.
+      destruct H0 as [?|[Hex|[Hex|Hex]]]; subst; auto.
+      + apply Exists_singl in Hex.
+        eapply IHHnormed1 in Hex as [?|[y [ck' [? [? ?]]]]]; auto 8.
+        right. exists y. exists ck'. auto 8.
+      + apply Exists_singl in Hex.
+        eapply IHHnormed2 in Hex as [?|[y [ck' [? [? ?]]]]]; auto 8.
+        right. exists y. exists ck'. auto 8.
+      + eapply wc_normalized_cexp_clockof_free_in with (x:=x) in Hnormed1 as [?|?]; eauto 8.
+        rewrite Hsingl0; repeat constructor; auto.
+    - (* merge *)
+      apply Forall_singl in H6. apply Forall_singl in H7.
+      simpl in *. symmetry in H11, H12. rewrite app_nil_r in H11, H12.
+      repeat singleton_length.
+      apply Forall_singl in H9; apply Forall_singl in H10; subst.
+      destruct H1 as [Hex|[Hex|[Hex|Hex]]]; subst; auto.
+      + eapply wc_normalized_lexp_Is_free_left in H as [?|[y [ck' [? [? ?]]]]]; eauto 10.
+      + apply Exists_singl in Hex.
+        eapply IHHnormed1 in Hex as [?|[y [ck' [? [? ?]]]]]; eauto 11.
+      + apply Exists_singl in Hex.
+        eapply IHHnormed2 in Hex as [?|[y [ck' [? [? ?]]]]]; eauto 11.
+      + eapply wc_normalized_cexp_clockof_free_in with (x:=x) in Hnormed1 as [?|[y [ck' [? [? ?]]]]]; eauto 11.
+        rewrite Hsingl0; repeat constructor; auto.
+    - (* lexp *)
+      eapply wc_normalized_lexp_Is_free_left in Hex; eauto.
+  Qed.
+
+  Lemma wc_untupled_eq_Is_free_left : forall G vars equ,
+      untupled_equation equ ->
+      wc_equation G vars equ ->
+      forall x, Exists (Is_free_left_ck x) (snd equ) ->
+           Exists (Is_free_left x) (snd equ) \/
+           exists y, exists ck', Exists (Is_free_left y) (snd equ) /\ In (y, ck') vars /\ Is_free_in_clock x ck'.
+  Proof.
+    intros * Hunt Hwc ? Hex; inv Hunt; simpl in *;
+      apply Exists_singl in Hex; destruct Hwc as [Hwc _]; apply Forall_singl in Hwc.
+    - (* app *)
+      inv Hwc. inv Hex. eapply wc_normalized_lexps_Is_free_left in H; eauto.
+      apply Exists_exists in H as [e [Hin [Hfree|[y [ck' [Hfree [Hin' Hfree']]]]]]].
+      + left. repeat constructor.
+        apply Exists_exists; eauto.
+      + right. exists y. exists ck'. repeat split; auto.
+        repeat constructor. apply Exists_exists; eauto.
+    - (* app (reset) *)
+      inv Hwc. inv Hex. inv H1; simpl in *; eauto.
+      + inv H2. destruct H1 as [?|?]; subst; eauto.
+        eapply wc_normalized_lexp_Is_free_left in H8 as [?|[y [ck' [? [? ?]]]]]; eauto 10.
+      + eapply wc_normalized_lexps_Is_free_left in H; eauto.
+        apply Exists_exists in H as [e [Hin [Hfree|[y [ck' [Hfree [Hin' Hfree']]]]]]].
+        * left. do 2 constructor. right.
+          apply Exists_exists; eauto.
+        * right. exists y. exists ck'. repeat split; auto.
+          do 2 constructor. right. apply Exists_exists; eauto.
+    - (* fby *)
+      inv Hwc. inv Hex.
+      simpl in *. rewrite app_nil_r in *. inv H6; inv H11. inv H7; inv H11.
+      destruct ann0 as (ty&ck&name); unfold clock_of_nclock, stripname in *; simpl in *.
+      apply Forall_singl in H4.
+      destruct H2 as [Hex|Hex]; apply Exists_singl in Hex.
+      + eapply wc_normalized_lexp_Is_free_left in Hex as [?|[y [ck' [? [? ?]]]]]; eauto 10.
+      + eapply wc_normalized_lexp_clockof_free_in in H as [?|[y [ck' [? [? ?]]]]]; eauto 10.
+        rewrite <- H9; auto.
+    - (* cexp *)
+      eapply wc_normalized_cexp_Is_free_left in H as [?|[y [ck' [? [? ?]]]]]; eauto 10.
+  Qed.
+
+  Fixpoint collect_free_in_clock (ck : clock) : list ident :=
+    match ck with
+    | Cbase => []
+    | Con ck' id _ => id::collect_free_in_clock ck'
+    end.
+
+  Definition collect_free_in_clocks (cks : list clock) : list ident :=
+    flat_map collect_free_in_clock cks.
+
+  Fact collect_free_in_clock_In : forall ck,
+      forall x, Is_free_in_clock x ck <-> In x (collect_free_in_clock ck).
+  Proof.
+    induction ck; intros x; split;
+      intros Hin; simpl in *; inv Hin; auto.
+    - right. rewrite <- IHck; auto.
+    - constructor.
+    - constructor. rewrite IHck; auto.
+  Qed.
+
+  Fact collect_free_in_clocks_In : forall cks,
+      Forall (fun ck => forall x, Is_free_in_clock x ck -> In x (collect_free_in_clocks cks)) cks.
+  Proof.
+    unfold collect_free_in_clocks.
+    induction cks; constructor.
+    - intros x Hfree.
+      rewrite flat_map_concat_map; simpl.
+      apply in_or_app; left. apply collect_free_in_clock_In; auto.
+    - eapply Forall_impl; eauto. intros ? Hin ? Hfree; simpl in *.
+      rewrite flat_map_concat_map in *; simpl.
+      apply in_or_app; right; eauto.
+  Qed.
+
+  Fact collect_free_in_clocks_In' : forall x cks,
+      In x (collect_free_in_clocks cks) <->
+      Exists (fun ck => Is_free_in_clock x ck) cks.
+  Proof.
+    unfold collect_free_in_clocks.
+    induction cks; simpl; split; intro Hin. 1,2:inv Hin.
+    - apply in_app_iff in Hin as [Hin|Hin].
+      + left. rewrite collect_free_in_clock_In; auto.
+      + right. rewrite <- IHcks; auto.
+    - rewrite in_app_iff. inv Hin.
+      + left. rewrite <- collect_free_in_clock_In; auto.
+      + right. rewrite IHcks; auto.
+  Qed.
+
+  Fact In_anon_streams_nclocksof_normalized : forall G vars id ck es,
+      Forall normalized_lexp es ->
+      Forall (wc_exp G vars) es ->
+      In (id, ck) (anon_streams (nclocksof es)) ->
+      Exists (fun e => exists ty, e = Evar id (ty, (ck, Some id))) es.
+  Proof.
+    intros * Hnormed Hwc Hin.
+    unfold anon_streams in Hin.
+    apply map_filter_In' in Hin as [[ck' id'] [Hin Hx]].
+    destruct id'; inv Hx.
+    unfold nclocksof in Hin. rewrite flat_map_concat_map, in_concat in Hin.
+    destruct Hin as [ncks [Hin Hin']]. simpl_In.
+    eapply Forall_forall in Hnormed; eauto.
+    eapply Forall_forall in Hwc; eauto.
+    inv Hnormed; inv Hwc; simpl in Hin.
+    1-6: destruct Hin as [Hin|Hin]; inv Hin.
+    apply Exists_exists. eexists; eauto.
+  Qed.
+
+  (*
+    If an equation is well-clocked on a clock ck, the variables in ck can appear
+    * defined by this very equation (due to the app rule)
+    * in the expression to the right of the equation
+    * "pulled-in" by other variables appearing in the expression
+   *)
+
+  Fact wc_untupled_equation_clockof_free_in : forall G vars xs es,
+      wc_global G ->
+      NoDupMembers vars ->
+      untupled_equation (xs, es) ->
+      wc_equation G vars (xs, es) ->
+      Forall (fun x => forall ck, In (x, ck) vars ->
+                          forall ckid, Is_free_in_clock ckid ck ->
+                                  In ckid xs \/
+                                  Exists (Is_free_left ckid) es \/
+                                  Exists (fun e => exists y, exists ck', Is_free_left y e
+                                                            /\ In (y, ck') vars
+                                                            /\ Is_free_in_clock ckid ck') es
+             ) xs.
+  Proof with eauto.
+    intros * HwcG Hndup Hunt (Hwc1&Hwc2&Hwc3).
+    inv Hunt.
+    - (* app *)
+      apply Forall_singl in Hwc1. inv Hwc1.
+      simpl in *; rewrite app_nil_r in *.
+      eapply WellInstantiated_is_free_in with (inputs:=collect_free_in_clocks (clocksof es0)) in H5; eauto. clear H6.
+      2: { specialize (collect_free_in_clocks_In (clocksof es0)) as Hcoll.
+           rewrite clocksof_nclocksof, Forall_map in Hcoll.
+           eapply Forall_impl; eauto. intros [? ?] Hin ? Hfree.
+           rewrite clocksof_nclocksof; eauto. }
+      assert (Forall (fun x => exists a, In a lann0 /\
+                                 forall ck, In (x, ck) vars ->
+                                       forall ckid, Is_free_in_clock ckid ck ->
+                                               In ckid xs \/
+                                               Exists (Is_free_left ckid) [Eapp f es0 None lann0] \/
+                                               Exists (fun e => exists y, exists ck', Is_free_left y e /\
+                                                                         In (y, ck') vars /\
+                                                                         Is_free_in_clock ckid ck') [Eapp f es0 None lann0]
+                     ) xs) as Hf'.
+      2:{ eapply Forall_impl; eauto. intros; simpl in *.
+          destruct H as [? [_ ?]]; eauto. }
+      eapply Forall2_ignore1' with (xs0:=xs) in H5. 2:(apply Forall2_length in Hwc2; solve_length).
+      rewrite Forall2_map_2 in Hwc3. rewrite Forall2_map_2 in H5.
+      eapply Forall2_Forall2 in H5; [|eapply Hwc3].
+      eapply Forall2_ignore2, Forall2_impl_In; [|eapply H5].
+      intros ? [? [ck' name]] Hina Hinb [Hvar Hin] ? Hvar' ? Hfree.
+      assert (ck' = ck); subst.
+      { eapply NoDupMembers_det in Hndup; eauto. }
+      eapply Hin in Hfree as [Hin'|[Hin'|Hin']]; clear Hin.
+      + eapply collect_free_in_clocks_In' in Hin'.
+        eapply wc_normalized_lexps_clocksof_free_in in Hin'...
+        apply Exists_exists in Hin' as [e [Hin [Hex|[y [ck' [Hex [Hin' Hfree]]]]]]].
+        * right. left. repeat constructor. apply Exists_exists. eexists...
+        * right. right. repeat constructor.
+          exists y. exists ck'. repeat split; auto. constructor. apply Exists_exists. eexists...
+      + simpl_In. destruct x as [id ck'].
+        eapply In_anon_streams_nclocksof_normalized in H1...
+        right. left. repeat constructor.
+        rewrite Exists_exists in *. destruct H1 as [e [? [? ?]]].
+        exists e; subst; auto.
+      + left. apply in_map_iff in Hin' as [[? ?] [? Hin]]; subst; simpl.
+        unfold anon_streams in Hin. apply map_filter_In' in Hin as [[? [?|]] [Hin Hx]]; inv Hx.
+        eapply Forall2_ignore1, Forall_forall in Hwc2 as [? [? ?]]; eauto.
+        inv H1; auto.
+    - (* app (reset) *)
+      apply Forall_singl in Hwc1. inv Hwc1.
+      simpl in *; rewrite app_nil_r in *.
+      eapply WellInstantiated_is_free_in with (ins:=(nclocksof es0)) (inputs:=collect_free_in_clocks (clocksof es0)) in H5; eauto. clear H6.
+      2: { specialize (collect_free_in_clocks_In (clocksof es0)) as Hcoll.
+           rewrite clocksof_nclocksof, Forall_map in Hcoll.
+           eapply Forall_impl; eauto. intros [? ?] Hin ? Hfree.
+           rewrite clocksof_nclocksof; eauto. }
+      assert (Forall (fun x0 => exists a, In a lann0 /\
+                                  forall ck, In (x0, ck) vars ->
+                                        forall ckid, Is_free_in_clock ckid ck ->
+                                                In ckid xs \/
+                                                Exists (Is_free_left ckid) [Eapp f es0 (Some (Evar x (ty, cl))) lann0] \/
+                                                Exists (fun e => exists y, exists ck', Is_free_left y e /\
+                                                                          In (y, ck') vars /\
+                                                                          Is_free_in_clock ckid ck') [Eapp f es0 (Some (Evar x (ty, cl)))lann0]
+                     ) xs) as Hf'.
+      2:{ solve_forall. destruct H1 as [? [_ ?]]; eauto. }
+      eapply Forall2_ignore1' with (xs0:=xs) in H5. 2:(apply Forall2_length in Hwc2; solve_length).
+      rewrite Forall2_map_2 in Hwc3. rewrite Forall2_map_2 in H5.
+      eapply Forall2_Forall2 in H5; [|eapply Hwc3].
+      eapply Forall2_ignore2, Forall2_impl_In; [|eapply H5].
+      intros ? [? [ck' name]] Hina Hinb [Hvar Hin] ? Hvar' ? Hfree.
+      assert (ck' = ck); subst.
+      { eapply NoDupMembers_det in Hndup; eauto. }
+      eapply Hin in Hfree as [Hin'|[Hin'|Hin']]; clear Hin.
+      + eapply collect_free_in_clocks_In' in Hin'.
+        eapply wc_normalized_lexps_clocksof_free_in in Hin'...
+        apply Exists_exists in Hin' as [e [Hin [Hex|[y [ck' [Hex [Hin' Hfree]]]]]]].
+        * right. left. do 2 constructor. right. apply Exists_exists. eexists...
+        * right. right. repeat constructor.
+          exists y. exists ck'. repeat split; auto. constructor. right. apply Exists_exists. eexists...
+      + simpl_In. destruct x0 as [id ck'].
+        eapply In_anon_streams_nclocksof_normalized in H1...
+        right. left. do 2 constructor. right.
+        rewrite Exists_exists in *. destruct H1 as [e [? [? ?]]].
+        exists e; subst; auto.
+      + left. apply in_map_iff in Hin' as [[? ?] [? Hin]]; subst; simpl.
+        unfold anon_streams in Hin. apply map_filter_In' in Hin as [[? [?|]] [Hin Hx]]; inv Hx.
+        eapply Forall2_ignore1, Forall_forall in Hwc2 as [? [? ?]]; eauto.
+        inv H1; auto.
+    - (* fby *)
+      clear Hwc2. simpl in *.
+      constructor; auto.
+      intros ck Hin ? Hfree.
+      apply Forall_singl in Hwc1. apply Forall2_singl in Hwc3.
+      destruct ann0 as [ty [ck' name]].
+      assert (ck' = ck); subst.
+      { eapply NoDupMembers_det in Hndup; eauto. }
+      right. inv Hwc1.
+      clear H2 H5 H7. apply Forall_singl in H4.
+      simpl in H6; rewrite app_nil_r, Forall2_eq in H6.
+      eapply wc_normalized_lexp_clockof_free_in in H4 as [Hex|[y [ck' [Hfree' [Hin' Hex]]]]]; eauto.
+      2:rewrite <- H6; auto.
+      right. left. exists y. exists ck'. repeat split; auto.
+    - (* cexp *)
+      clear Hwc2.
+      constructor; auto.
+      intros ck Hin ? Hfree.
+      apply Forall_singl in Hwc1.
+      simpl in Hwc3; rewrite app_nil_r in Hwc3. inv Hwc3; inv H4.
+      assert (y = ck); subst.
+      { eapply NoDupMembers_det in Hndup; eauto. }
+      right. eapply wc_normalized_cexp_clockof_free_in in Hwc1 as [HEx|[y [ck' [Hfree' [Hin' Hex']]]]]; eauto.
+      2:rewrite <- H2; auto.
+      right. left. exists y. exists ck'. repeat split; auto.
+  Qed.
+
+  Lemma wc_untupled_equations_clockof_causal : forall G vars inputs eqs,
+      incl inputs vars ->
+      NoDupMembers vars ->
+      Forall untupled_equation eqs ->
+      wc_global G ->
+      wc_env inputs ->
+      Forall (wc_equation G vars) eqs ->
+      Is_causal (map fst inputs) eqs ->
+      Forall (fun x => forall ck, In (x, ck) vars ->
+                          forall ckid, Is_free_in_clock ckid ck ->
+                                  In ckid (vars_defined eqs) \/
+                                  In ckid (map fst inputs)) (vars_defined eqs).
+  Proof with eauto.
+    induction eqs; intros Hincl Hndup Hunt HwcG Hwenv Hwc Hcaus; inv Hunt; inv Hwc; inv Hcaus; simpl; auto.
+    apply Forall_app; split; eauto.
+    - destruct a as [xs es].
+      specialize (wc_untupled_equation_clockof_free_in _ _ _ _ HwcG Hndup H1 H3) as Hfree.
+      eapply Forall_impl; eauto. clear Hfree. intros; simpl in *.
+      rewrite in_app_iff, or_assoc.
+      specialize (H _ H0 _ H7) as [?|[?|Hfree]]; auto.
+      apply Exists_exists in Hfree as [e [Hin [? [? [Hfree [Hinvars Hfree']]]]]].
+      assert (Exists (Is_free_left x) es) as Hex.
+      { rewrite Exists_exists. exists e; auto. }
+      apply H6 in Hex as [Hex|Hex].
+      + eapply IHeqs in H2...
+        eapply Forall_forall in H2...
+      + right. right.
+        rewrite <- fst_InMembers in *. eapply incl_NoDup_In in Hex...
+        eapply wc_env_Is_free_in_clock_In...
+    - eapply IHeqs in H5; eauto.
+      solve_forall. rewrite in_app_iff. eapply H0 in H4 as [?|?]...
+  Qed.
+
+  Lemma Is_causal_Is_causal_ck : forall G vars inputs eqs,
+      incl inputs vars ->
+      NoDupMembers vars ->
+      Forall untupled_equation eqs ->
+      wc_global G ->
+      wc_env inputs ->
+      Forall (wc_equation G vars) eqs ->
+      Is_causal (map fst inputs) eqs ->
+      Is_causal_ck (map fst inputs) eqs.
+  Proof with eauto.
+    induction eqs; intros Hincl Hndup Hunt HwcG Hwenv Hwc Hcaus; inv Hunt; inv Hwc; inv Hcaus; simpl; auto.
+    constructor; auto. clear IHeqs.
+    intros x Hex.
+    eapply wc_untupled_eq_Is_free_left in Hex as [?|[y [ck' [? [? ?]]]]]; eauto.
+    destruct a as [xs es].
+    eapply H6 in H as [H|H].
+    - specialize (wc_untupled_equations_clockof_causal _ _ _ _ Hincl Hndup H2 HwcG Hwenv H4 H5) as Heqs.
+      eapply Forall_forall in Heqs; eauto.
+    - right. rewrite <- fst_InMembers in *.
+      eapply incl_NoDup_In, wc_env_Is_free_in_clock_In in H...
+  Qed.
+
+  (** ** Additional properties of Is_causal_ck *)
+
+  Lemma Is_causal_ck_incl : forall ins1 ins2 eqs,
+      incl ins1 ins2 ->
+      Is_causal_ck ins1 eqs ->
+      Is_causal_ck ins2 eqs.
+  Proof.
+    induction eqs; intros Hincl Hcaus; inv Hcaus; auto.
+    constructor; auto.
+    intros ? Hex. apply H2 in Hex as [?|Hex]; auto.
+  Qed.
+
+  Instance causal_ck_Proper:
+    Proper (@Permutation ident ==> @eq (list equation) ==> @Basics.impl)
+           Is_causal_ck.
+  Proof.
+    intros ? ? Hp1 ? ? Heq Hcaus; subst.
+    eapply Is_causal_ck_incl; eauto.
+    rewrite Hp1. reflexivity.
+  Qed.
+
+  Lemma Is_causal_ck_appr : forall eqs eqs' ins,
+      Is_causal_ck ins (eqs ++ eqs') ->
+      Is_causal_ck ins eqs'.
+  Proof.
+    induction eqs; intros * Hcaus; simpl in *; auto.
+    inv Hcaus; eauto.
+  Qed.
+
+  Lemma Is_causal_ck_appl : forall eqs eqs' ins,
+      Is_causal_ck ins (eqs ++ eqs') ->
+      Is_causal_ck (ins++vars_defined eqs') eqs.
+  Proof.
+    induction eqs; intros * Hcaus; simpl in *.
+    - constructor.
+    - inv Hcaus. eapply IHeqs in H1. constructor; auto.
+      intros x Hex. apply H2 in Hex.
+      rewrite vars_defined_app in Hex. rewrite in_app_iff in *.
+      destruct Hex as [[?|?]|?]; auto.
+  Qed.
+
+  Lemma Is_causal_ck_app : forall eqs eqs' ins,
+      Is_causal_ck ins eqs' ->
+      Is_causal_ck (ins++vars_defined eqs') eqs ->
+      Is_causal_ck ins (eqs ++ eqs').
+  Proof.
+    induction eqs; intros * Hcaus1 Hcaus2; simpl in *.
+    - auto.
+    - inv Hcaus2.
+      constructor; auto.
+      intros x Hex. apply H2 in Hex.
+      rewrite vars_defined_app. rewrite in_app_iff in *.
+      destruct Hex as [?|[?|?]]; auto.
+  Qed.
+
+  Lemma Is_causal_ck_app' : forall ins eqs1 eqs2,
+      Is_causal_ck ins eqs1 ->
+      Is_causal_ck ins eqs2 ->
+      Is_causal_ck ins (eqs1 ++ eqs2).
+  Proof.
+    intros * Hcaus1 Hcaus2.
+    eapply Is_causal_ck_app; eauto.
+    eapply Is_causal_ck_incl; eauto.
+    apply incl_appl, incl_refl.
+  Qed.
+
+  Lemma Is_causal_ck_Forall : forall inputs eqs,
+      Is_causal_ck inputs eqs ->
+      Forall (fun eq => forall x, Exists (Is_free_left_ck x) (snd eq) -> In x (vars_defined eqs) \/ In x inputs) eqs.
+  Proof.
+    induction eqs; intros Hcaus; auto.
+    inv Hcaus.
+    constructor.
+    - intros ? Hex. eapply H2 in Hex.
+      simpl. rewrite in_app_iff, or_assoc. destruct Hex; auto.
+    - apply IHeqs in H1. solve_forall.
+      apply H0 in H1. rewrite in_app_iff, or_assoc. destruct H1; auto.
+  Qed.
+
+  Lemma Is_causal_ck_Forall' : forall inputs eqs,
+      Forall (fun eq => forall x, Exists (Is_free_left_ck x) (snd eq) -> In x inputs) eqs ->
+      Is_causal_ck inputs eqs.
+  Proof.
+    induction eqs; intros Hcaus; auto.
+    inv Hcaus.
+    constructor; auto.
+  Qed.
+
+  Fixpoint collect_free_left_ck (e : exp) : list ident :=
+    let collect_free_lefts_ck := flat_map collect_free_left_ck in
+    match e with
+    | Econst _ => []
+    | Evar id (_, (ck, _)) => id::(collect_free_in_clock ck)
+    | Eunop _ e (_, (ck, _)) => (collect_free_left_ck e)++(collect_free_in_clock ck)
+    | Ebinop _ e1 e2 (_, (ck, _)) => (collect_free_left_ck e1)++(collect_free_left_ck e2)++(collect_free_in_clock ck)
+    | Efby e0s es anns =>
+      (collect_free_lefts_ck e0s)++(collect_free_in_clocks (map clock_of_nclock anns))
+    | Ewhen es id _ (_, (ck, _)) =>
+      id::(collect_free_lefts_ck es)++(collect_free_in_clock ck)
+    | Emerge id ets efs (_, (ck, _)) =>
+      id::(collect_free_lefts_ck ets)++(collect_free_lefts_ck efs)++(collect_free_in_clock ck)
+    | Eite e ets efs (_, (ck, _)) =>
+      (collect_free_left_ck e)++(collect_free_lefts_ck ets)++(collect_free_lefts_ck efs)++(collect_free_in_clock ck)
+    | Eapp _ es None _ =>
+      collect_free_lefts_ck es
+    | Eapp _ es (Some r) _ =>
+      (collect_free_lefts_ck es) ++ (collect_free_left_ck r)
+    end.
+
+  Definition collect_free_lefts_ck (es : list exp) :=
+    flat_map collect_free_left_ck es.
+
+  Lemma collect_free_left_ck_sound : forall e x,
+      In x (collect_free_left_ck e) <-> Is_free_left_ck x e.
+  Proof.
+    intros e x. split; intros H.
+    - induction e using exp_ind2; simpl in *. 9:destruct ro.
+      Local Ltac Forall_Exists_Exists H :=
+        rewrite in_flat_map' in H;
+        eapply Forall_Exists in H; [|eauto];
+        eapply Exists_Exists; [|eauto]; intros ? [? ?]; auto.
+      + (* const *) inv H.
+      + (* var *)
+        destruct a as [ty [ck name]].
+        inv H; auto. constructor. rewrite collect_free_in_clock_In; auto.
+      + (* unop *)
+        destruct a as [ty [ck name]].
+        rewrite in_app_iff, <- collect_free_in_clock_In in H. destruct H; auto.
+      + (* binop *)
+        destruct a as [ty [ck name]].
+        rewrite in_app_iff, in_app_iff, <- collect_free_in_clock_In in H. destruct H as [?|[?|?]]; auto.
+      + (* fby *)
+        rewrite in_app_iff in H. destruct H.
+        * constructor. left. Forall_Exists_Exists H.
+        * constructor. right. apply collect_free_in_clocks_In'; auto.
+      + (* when *)
+        destruct a as [tys [ck name]].
+        destruct H; auto. rewrite in_app_iff, <- collect_free_in_clock_In in H; destruct H; auto.
+        constructor. right. left. Forall_Exists_Exists H.
+      + (* merge *)
+        destruct a as [tys [ck name]].
+        destruct H; auto.
+        repeat rewrite in_app_iff in H. rewrite <- collect_free_in_clock_In in H.
+        destruct H as [?|[?|?]]; auto.
+        * constructor. right. left. Forall_Exists_Exists H.
+        * constructor. right. right. left. Forall_Exists_Exists H.
+      + (* ite *)
+        destruct a as [tys [ck name]].
+        repeat rewrite in_app_iff in H. rewrite <- collect_free_in_clock_In in H.
+        destruct H as [?|[?|[?|?]]]; auto.
+        * constructor. right. left. Forall_Exists_Exists H.
+        * constructor. right. right. left. Forall_Exists_Exists H.
+      + (* app (reset) *)
+        rewrite in_app_iff in H. destruct H as [?|?]; auto.
+        constructor. right. Forall_Exists_Exists H.
+      + (* app *)
+        constructor. Forall_Exists_Exists H.
+    - induction e using exp_ind2; simpl; inv H;
+        repeat rewrite in_app_iff.
+      Local Ltac Forall_Exists_Exists2 H :=
+        eapply Forall_Exists in H; [|eauto];
+        rewrite in_flat_map';
+        eapply Exists_Exists; [|eauto]; intros ? [? ?]; auto.
+      + (* var *)
+        destruct H1; subst; auto.
+        * left; auto.
+        * right. rewrite <- collect_free_in_clock_In; auto.
+      + (* unop *)
+        destruct H1; auto.
+        right. rewrite <- collect_free_in_clock_In; auto.
+      + (* binop *)
+        destruct H1 as [?|[?|?]]; auto.
+        right. right. rewrite <- collect_free_in_clock_In; auto.
+      + (* fby *)
+        rewrite collect_free_in_clocks_In'.
+        destruct H3; auto.
+        left. Forall_Exists_Exists2 H.
+      + (* when *)
+        simpl. rewrite in_app_iff, <- collect_free_in_clock_In.
+        destruct H2 as [?|[?|?]]; auto.
+        right. left. Forall_Exists_Exists2 H.
+      + (* merge *)
+        simpl. repeat rewrite in_app_iff. rewrite <- collect_free_in_clock_In.
+        destruct H3 as [?|[?|[?|?]]]; auto.
+        * right. left. Forall_Exists_Exists2 H.
+        * right. right. left. Forall_Exists_Exists2 H.
+      + (* ite *)
+        rewrite <- collect_free_in_clock_In.
+        destruct H3 as [?|[?|[?|?]]]; auto.
+        * right. left. Forall_Exists_Exists2 H.
+        * right. right. left. Forall_Exists_Exists2 H.
+      + (* app *)
+        Forall_Exists_Exists2 H3.
+      + (* app (reset) *)
+        inv H3; auto.
+        left. Forall_Exists_Exists2 H2.
+  Qed.
+
+  Corollary collect_free_lefts_ck_sound : forall es x,
+      In x (collect_free_lefts_ck es) <-> Exists (Is_free_left_ck x) es.
+  Proof.
+    intros es x.
+    unfold collect_free_lefts_ck. rewrite flat_map_concat_map.
+    split; intros.
+    - apply in_concat in H as [? [Hin ?]].
+      simpl_In. apply Exists_exists. exists x1. split; auto.
+      rewrite collect_free_left_ck_sound in Hin; auto.
+    - apply Exists_exists in H as [e [Hin Hfree]].
+      eapply incl_concat_map in Hin.
+      eapply Hin.
+      rewrite collect_free_left_ck_sound; auto.
+  Qed.
+
+  Fact causal_insert_early' : forall dom eqs inputs,
+      NoDup (vars_defined eqs++inputs) ->
+      Is_causal_ck inputs eqs ->
+      Forall (fun x => In x (vars_defined eqs) \/ In x inputs) dom ->
+      exists eqs1, exists eqs2,
+          eqs = eqs1 ++ eqs2 /\
+          Forall (fun x => In x (vars_defined eqs2) \/ In x inputs) dom /\
+          Forall (fun eq => not (Forall (fun x => Exists (Is_free_left_ck x) (snd eq)) dom)) eqs2.
+  Proof.
+    induction eqs; intros * Hndup Hcaus Hfree.
+    - exists []. exists []. repeat split; simpl; auto.
+    - destruct a as [xs' es']. inv Hcaus. simpl in *.
+      specialize (in_dec ident_eq_dec) as Hdec.
+      rewrite <- app_assoc in Hndup.
+      assert (NoDup (vars_defined eqs++inputs)) as Hndup'.
+      { apply NoDup_app_r in Hndup; auto. }
+      specialize (IHeqs _ Hndup' H1).
+      specialize (Forall_Exists_dec (fun x => ~In x xs')) with (l:=dom) as [Hdom|Hdom].
+      { intros x. specialize (Hdec x xs') as [Hin|?]; auto. }
+      + assert (Forall (fun x => In x (vars_defined eqs) \/ In x inputs) dom) as Hdom'.
+        { solve_forall.
+          rewrite in_app_iff, or_assoc in H3. destruct H3 as [?|[?|?]]; auto. contradiction. }
+        specialize (IHeqs Hdom') as [eqs1 [eqs2 [? [? ?]]]]; subst.
+        exists ((xs', es')::eqs1). exists eqs2. repeat split; auto.
+      + exists []. eexists. repeat split; eauto.
+        assert (Exists (fun x => In x xs') dom) as Hdom'.
+        { eapply Exists_Exists; eauto.
+          intros ? Hin; simpl in Hin. apply not_not; auto.
+          apply ListDec.In_decidable. intros ? ?. apply decidable_eq_ident. } clear Hdom.
+        constructor; simpl.
+        * intro contra.
+          simpl_forall.
+          eapply Forall_Exists, Exists_exists in Hdom' as [? [_ [Hfree' Hxs']]]; eauto.
+          simpl in Hfree'. destruct Hfree' as [Hfree' _]. apply H2 in Hfree'.
+          eapply NoDup_app_In in Hndup; eauto.
+          eapply Hndup, in_or_app; auto.
+        * apply Is_causal_ck_Forall in H1.
+          solve_forall. intro contra.
+          solve_forall.
+          eapply Forall_Exists, Exists_exists in Hdom' as [? [? [Hfree' Hxs']]]; eauto.
+          simpl in Hfree'. destruct Hfree' as [Hfree' _].
+          apply H0 in Hfree'.
+          eapply NoDup_app_In in Hndup; eauto.
+          eapply Hndup, in_or_app; auto.
+  Qed.
+
+  Lemma causal_insert_early : forall inputs eqs xs es,
+      NoDup (vars_defined eqs++inputs) ->
+      Is_causal_ck inputs eqs ->
+      (forall x, Exists (Is_free_left_ck x) es -> In x (vars_defined eqs) \/ In x inputs) ->
+      exists eqs1, exists eqs2,
+          eqs = eqs1 ++ eqs2 /\
+          Is_causal_ck inputs (eqs1 ++ (xs, es) :: eqs2) /\
+          Forall (fun eq => (forall x, Exists (Is_free_left_ck x) es -> Exists (Is_free_left_ck x) (snd eq)) ->
+                         In eq eqs1) eqs.
+  Proof.
+    intros * Hndup Hcaus Hfree.
+    assert (Forall (fun x => In x (vars_defined eqs) \/ In x inputs) (collect_free_lefts_ck es)) as Hfree'.
+    { solve_forall. eapply Hfree. rewrite collect_free_lefts_ck_sound in H; auto. }
+    eapply causal_insert_early' in Hfree' as [eqs1 [eqs2 [? [Hex Hf]]]]; eauto; subst.
+    exists eqs1. exists eqs2. repeat split; auto.
+    apply Is_causal_ck_app.
+    - constructor; eauto.
+      eapply Is_causal_ck_appr in Hcaus; auto.
+      intros ? Hex'. rewrite Forall_forall in Hex.
+      rewrite <- collect_free_lefts_ck_sound in Hex'; eauto.
+    - apply Is_causal_ck_appl in Hcaus.
+      eapply Is_causal_ck_incl; [|eauto].
+      simpl. apply incl_appr', incl_appr, incl_refl.
+    - apply Forall_app; split.
+      + apply Forall_forall. intros; auto.
+      + solve_forall; simpl in *. exfalso.
+        apply H0, Forall_forall. intros ? Hin.
+        apply H1. rewrite collect_free_lefts_ck_sound in Hin; eauto.
+  Qed.
+
+  (** ** Causality of the second phase of normalization *)
+
+  (** *** Recover info about the init equations in the state *)
+
+  Definition st_inits (st : fresh_st (Op.type * clock * bool)) :=
+    map (fun '(id, ((_, ck), _)) => (id, ck)) (filter (fun '(_, (ty, _, b)) => b && (ty ==b Op.bool_type)) (st_anns st)).
+
+  Fact st_follows_inits_incl : forall st st',
+      st_follows st st' ->
+      incl (st_inits st) (st_inits st').
+  Proof.
+    intros * Hfollows.
+    eapply st_follows_incl in Hfollows.
+    unfold st_inits.
+    apply incl_map, incl_filter; auto.
+  Qed.
+
+  Fact st_inits_find_Some : forall st x (ck : nclock) p,
+      find (fun '(_, (ty, ck', isinit)) => isinit && (ck' ==b fst ck) && (ty ==b Op.bool_type)) (st_anns st) = Some (x, p) ->
+      In (x, (fst ck)) (st_inits st).
+  Proof.
+    intros * Hfind.
+    apply find_some in Hfind as [Hin Hf].
+    destruct p as [[ty ck'] isinit].
+    repeat rewrite Bool.andb_true_iff in Hf. destruct Hf as [[Hty Hck] ?]; auto.
+    unfold st_inits. rewrite in_map_iff. exists (x, (ty, ck', isinit)); split; auto.
+    - rewrite clock_eqb_eq in Hck. f_equal; auto.
+    - rewrite filter_In; split; auto.
+      rewrite Hty, H; auto.
+  Qed.
+
+  Fact st_inits_find_None : forall st (ck : nclock),
+      find (fun '(_, (ty, ck', isinit)) => isinit && (ck' ==b fst ck) && (ty ==b Op.bool_type)) (st_anns st) = None ->
+      ~In (fst ck) (map snd (st_inits st)).
+  Proof.
+    intros * Hfind.
+    intro contra. unfold st_inits in contra. repeat simpl_In; simpl in *; inv H0; subst.
+    apply filter_In in H1 as [Hin Heq].
+    eapply find_none in Hfind; eauto. simpl in *.
+    apply Bool.andb_true_iff in Heq as [Hb Hty]; subst; simpl in Hfind.
+    rewrite Hty, equiv_decb_refl in Hfind; simpl in Hfind. congruence.
+  Qed.
+
+  Fact fresh_ident_false_st_inits : forall (st st' : fresh_st (Op.type * clock * bool)) a id,
+      fresh_ident (a, false) st = (id, st') ->
+      st_inits st' = st_inits st.
+  Proof.
+    intros * Hfresh.
+    unfold st_inits. destruct a as [ty ck].
+    apply fresh_ident_anns in Hfresh. rewrite Hfresh.
+    simpl; auto.
+  Qed.
+
+  Fact fresh_ident_true_st_inits : forall st st' ck id,
+      fresh_ident ((Op.bool_type, ck), true) st = (id, st') ->
+      st_inits st' = (id, ck)::st_inits st.
+  Proof.
+    intros * Hfresh.
+    unfold st_inits.
+    apply fresh_ident_anns in Hfresh. rewrite Hfresh.
+    simpl. rewrite equiv_decb_refl; auto.
+  Qed.
+
+  Fact init_var_for_clock_In_st_inits : forall ck x eqs' st st',
+      init_var_for_clock ck st = (x, eqs', st') ->
+      In (x, ck) (st_inits st').
+  Proof.
+    intros * Hinit.
+    eapply init_var_for_clock_In in Hinit.
+    unfold st_inits.
+    simpl_In. exists (x, (Op.bool_type, ck, true)); split; auto.
+    rewrite filter_In. split; auto.
+    rewrite equiv_decb_refl; auto.
+  Qed.
+
+  Fact add_whens_Is_free_left : forall ck ty c,
+      forall x, Is_free_left_ck x (add_whens (Econst c) ty ck) ->
+           Is_free_in_clock x ck.
+  Proof.
+    induction ck; intros * Hfree; inv Hfree.
+    destruct H0; subst; auto.
+    - constructor.
+    - destruct H; auto.
+      apply Exists_singl in H.
+      constructor; eauto.
+  Qed.
+
+  (** *** Small properties on the clocking of generated equations *)
+
+  Fact init_var_for_clock_clocksof : forall ck id eqs' st st',
+      init_var_for_clock ck st = (id, eqs', st') ->
+      Forall (fun eq => clocksof (snd eq) = [ck]) eqs'.
+  Proof.
+    intros * Hinit.
+    unfold init_var_for_clock in Hinit.
+    destruct (find _ _); repeat inv_bind.
+    - destruct p; inv Hinit; auto.
+    - destruct (fresh_ident _ _); inv Hinit; auto.
+  Qed.
+
+  Fact fby_iteexp_clocksof : forall e0 e ty ck name e' eqs' st st',
+      fby_iteexp e0 e (ty, (ck, name)) st = (e', eqs', st') ->
+      Forall (fun eq => clocksof (snd eq) = [ck]) eqs'.
+  Proof.
+    intros * Hfby; simpl in *.
+    destruct (is_constant _); repeat inv_bind; constructor; auto.
+    eapply init_var_for_clock_clocksof; eauto.
+  Qed.
+
+  (** *** Perservation of weak validity *)
+
+  Fact init_var_for_clock_weak_valid : forall inputs eqs ck x eqs' st st',
+      weak_valid_after st (ps_from_list (vars_defined eqs++inputs)) ->
+      init_var_for_clock ck st = (x, eqs', st') ->
+      weak_valid_after st' (ps_from_list (vars_defined (eqs++eqs')++inputs)).
+  Proof.
+    intros * Hweak Hinit. unfold init_var_for_clock in Hinit.
+    destruct (find _ _).
+    - destruct p; inv Hinit. rewrite app_nil_r; auto.
+    - destruct (fresh_ident _ _) eqn:Hfresh. inv Hinit.
+      rewrite vars_defined_app; simpl.
+      eapply fresh_ident_weak_valid in Hfresh; eauto.
+      rewrite (Permutation_app_comm (vars_defined _)); simpl.
+      rewrite <- add_ps_from_list_cons; auto.
+  Qed.
+
+  Fact fby_iteexp_weak_valid : forall inputs eqs e0 e ty ck name e' eqs' st st',
+      weak_valid_after st (ps_from_list (vars_defined eqs++inputs)) ->
+      fby_iteexp e0 e (ty, (ck, name)) st = (e', eqs', st') ->
+      weak_valid_after st' (ps_from_list (vars_defined (eqs++eqs')++inputs)).
+  Proof.
+    intros * Hweak Hfby.
+    unfold fby_iteexp in Hfby.
+    destruct (is_constant e0); repeat inv_bind.
+    - rewrite app_nil_r; auto.
+    - eapply init_var_for_clock_weak_valid in H; eauto.
+      eapply fresh_ident_weak_valid in H0; eauto.
+      rewrite vars_defined_app in *; simpl.
+      rewrite <- Permutation_middle; simpl. rewrite <- add_ps_from_list_cons; auto.
+  Qed.
+
+  Fact fby_equation_weak_valid : forall to_cut inputs eq eqs eqs' st st',
+      weak_valid_after st (ps_from_list (vars_defined (eq::eqs)++inputs)) ->
+      fby_equation to_cut eq st = (eqs', st') ->
+      weak_valid_after st' (ps_from_list (vars_defined (eqs++eqs')++inputs)).
+  Proof.
+    intros * Hweak Hfby.
+    inv_fby_equation Hfby to_cut eq.
+    - destruct x2 as [ty [ck name]]; repeat inv_bind.
+      eapply fby_iteexp_weak_valid with (eqs:=([x], [Efby [x0] [x1] [(ty, (ck, name))]])::eqs) in H; simpl in *; eauto.
+      destruct (PS.mem _ _); repeat inv_bind.
+      + eapply fresh_ident_weak_valid in H0; eauto.
+        rewrite vars_defined_app in *; simpl in *.
+        rewrite <- Permutation_middle, <- Permutation_middle, perm_swap; simpl.
+        rewrite <- add_ps_from_list_cons; auto.
+      + rewrite vars_defined_app in *; simpl in *.
+        rewrite <- Permutation_middle; auto.
+    - rewrite vars_defined_app; simpl.
+      rewrite app_nil_r, (Permutation_app_comm (vars_defined _)); auto.
+  Qed.
+
+  (** A weaker version, but useful for us *)
+
+  Fact init_var_for_clock_weak_valid' : forall ck x eqs' st st' aft,
+      weak_valid_after st aft ->
+      init_var_for_clock ck st = (x, eqs', st') ->
+      weak_valid_after st' aft.
+  Proof.
+    intros * Hweak Hinit. unfold init_var_for_clock in Hinit.
+    destruct (find _ _).
+    - destruct p; inv Hinit; auto.
+    - destruct (fresh_ident _ _) eqn:Hfresh. inv Hinit.
+      eapply Facts.fresh_ident_weak_valid' in Hfresh; eauto.
+  Qed.
+
+  Fact fby_iteexp_weak_valid' : forall e0 e ty ck name e' eqs' st st' aft,
+      weak_valid_after st aft ->
+      fby_iteexp e0 e (ty, (ck, name)) st = (e', eqs', st') ->
+      weak_valid_after st' aft.
+  Proof.
+    intros * Hweak Hfby. unfold fby_iteexp in Hfby.
+    destruct (is_constant e0); repeat inv_bind; auto.
+    eapply init_var_for_clock_weak_valid' in H; eauto.
+    eapply Facts.fresh_ident_weak_valid' in H0; eauto.
+  Qed.
+
+  (** *** With weak validity, we can get NoDup results *)
+
+  Fact init_var_for_clock_NoDup : forall inputs eqs ck x eqs' st st',
+      NoDup (vars_defined eqs++inputs) ->
+      weak_valid_after st (ps_from_list (vars_defined eqs++inputs)) ->
+      init_var_for_clock ck st = (x, eqs', st') ->
+      NoDup (vars_defined (eqs++eqs')++inputs).
+  Proof.
+    intros * Hndup Hweak Hinit. unfold init_var_for_clock in Hinit.
+    destruct (find _ _).
+    - destruct p; inv Hinit. rewrite app_nil_r; auto.
+    - destruct (fresh_ident _ _) eqn:Hfresh. inv Hinit.
+      rewrite vars_defined_app; simpl.
+      rewrite (Permutation_app_comm (vars_defined _)); simpl.
+      constructor; auto.
+      eapply fresh_ident_weak_valid_nIn in Hfresh; eauto.
+      rewrite ps_from_list_In in Hfresh; auto.
+  Qed.
+
+  Fact fby_iteexp_NoDup : forall inputs eqs e0 e ty ck name e' eqs' st st',
+      NoDup (vars_defined eqs++inputs) ->
+      weak_valid_after st (ps_from_list (vars_defined eqs++inputs)) ->
+      fby_iteexp e0 e (ty, (ck, name)) st = (e', eqs', st') ->
+      NoDup (vars_defined (eqs++eqs')++inputs).
+  Proof.
+    intros * Hnd Hweak Hfby. unfold fby_iteexp in Hfby.
+    destruct (is_constant _); repeat inv_bind.
+    - rewrite app_nil_r; auto.
+    - assert (Hnd1:=H). eapply init_var_for_clock_weak_valid in H; eauto.
+      eapply init_var_for_clock_NoDup in Hnd1; eauto.
+      rewrite vars_defined_app in *; simpl.
+      rewrite <- Permutation_middle; simpl. constructor; auto.
+      eapply fresh_ident_weak_valid_nIn in H0; eauto.
+      rewrite ps_from_list_In in H0; auto.
+  Qed.
+
+  (** *** Also, ids in the valid state dont appear in the vars defined by generated equations *)
+
+  Fact init_var_for_clock_weak_valid_nIn : forall ck x eqs' st st' id aft,
+      PS.In id aft ->
+      weak_valid_after st aft ->
+      init_var_for_clock ck st = (x, eqs', st') ->
+      ~In id (vars_defined eqs').
+  Proof.
+    intros * Hin Hweak Hinit contra.
+    unfold init_var_for_clock in Hinit. destruct (find _ _).
+    - destruct p; inv Hinit; auto.
+    - destruct (fresh_ident _) eqn:Hfresh; inv Hinit; simpl in *.
+      inv contra; auto.
+      eapply fresh_ident_weak_valid_nIn in Hfresh; eauto.
+  Qed.
+
+  Fact fby_iteexp_weak_valid_nIn : forall e0 e a e' eqs' st st' id aft,
+      PS.In id aft ->
+      weak_valid_after st aft ->
+      fby_iteexp e0 e a st = (e', eqs', st') ->
+      ~In id (vars_defined eqs').
+  Proof.
+    intros * Hnin Hvalid Hfby contra. destruct a as [ty [ck name]].
+    unfold fby_iteexp in Hfby.
+    destruct (is_constant _); repeat inv_bind; simpl in *; auto.
+    inv contra.
+    - eapply fresh_ident_weak_valid_nIn in H0; eauto.
+      eapply init_var_for_clock_weak_valid' in H; eauto.
+    - eapply init_var_for_clock_weak_valid_nIn in H; eauto.
+  Qed.
+
+  (** *** And finally, we can keep info about what isn't in st_inits *)
+
+  Fact init_var_for_clock_weak_valid_nIn_st_inits : forall ck x eqs' st st' id aft,
+      PS.In id aft ->
+      weak_valid_after st aft ->
+      ~In id (map fst (st_inits st)) ->
+      init_var_for_clock ck st = (x, eqs', st') ->
+      ~In id (map fst (st_inits st')).
+  Proof.
+    intros * Hin Hweak Hnin Hinit.
+    unfold init_var_for_clock in Hinit. destruct (find _ _).
+    - destruct p; inv Hinit; auto.
+    - destruct (fresh_ident _ _) eqn:Hfresh; inv Hinit.
+      assert (Hnin':=Hfresh). eapply fresh_ident_weak_valid_nIn in Hnin'; eauto.
+      eapply fresh_ident_true_st_inits in Hfresh. rewrite Hfresh.
+      intro contra. inv contra; auto.
+  Qed.
+
+  Fact fby_iteexp_weak_valid_nIn_st_inits : forall e0 e a e' eqs' st st' id aft,
+      PS.In id aft ->
+      weak_valid_after st aft ->
+      ~In id (map fst (st_inits st)) ->
+      fby_iteexp e0 e a st = (e', eqs', st') ->
+      ~In id (map fst (st_inits st')).
+  Proof.
+    intros * Hin Hweak Hnin Hfby. destruct a as [ty [ck name]].
+    unfold fby_iteexp in Hfby. destruct (is_constant _); repeat inv_bind; auto.
+    eapply init_var_for_clock_weak_valid_nIn_st_inits in H; eauto.
+    eapply fresh_ident_false_st_inits in H0. congruence.
+  Qed.
+
+  Fact fby_equation_weak_valid_nIn_st_inits : forall to_cut eq eqs' st st' id aft,
+      PS.In id aft ->
+      weak_valid_after st aft ->
+      ~In id (map fst (st_inits st)) ->
+      fby_equation to_cut eq st = (eqs', st') ->
+      ~In id (map fst (st_inits st')).
+  Proof.
+    intros * Hin Hweak Hnin Hfby.
+    inv_fby_equation Hfby to_cut eq.
+    destruct x2 as [ty [ck name]]; repeat inv_bind.
+    eapply fby_iteexp_weak_valid_nIn_st_inits with (a:=(ty, (ck, name))) in H; eauto.
+    destruct (PS.mem _ _); repeat inv_bind; auto.
+    eapply fresh_ident_false_st_inits in H0. congruence.
+  Qed.
+
+  (** *** Causality invariant
+      We have to talk about the causality of the whole set of equation
+      (since we will be inserting init equations early).a
+      The inveriant contains several part:
+      * Two general no-duplication hypothesis, respectively about the vars
+        defined by equations and about the st_inits
+      * A strengthened causality hypothesis : the set of equations is causal,
+        and the init equations appear before any equation on the same clock as them *)
+
+  Definition is_not_app (e : exp) :=
+    match e with
+    | Eapp _ _ _ _ => False
+    | _ => True
+    end.
+
+  Definition causal_inv inputs eqs (st : fresh_st (Op.type * clock * bool)) :=
+    NoDup (vars_defined eqs ++ inputs) /\
+    NoDup (map snd (st_inits st)) /\
+    exists ceqs, Permutation eqs ceqs /\
+            Is_causal_ck inputs ceqs /\
+            Forall (fun '(x, ck) => exists eqs1, exists eqs2, exists e,
+                              ceqs = eqs1 ++ ([x], [e]) :: eqs2 /\
+                              clockof e = [ck] /\
+                              Forall (fun eq => (exists e, snd eq = [e] /\
+                                                   is_not_app e /\
+                                                   clockof e = [ck]) ->
+                                             In eq eqs1) (eqs1++eqs2)) (st_inits st).
+
+  Instance causal_inv_Proper:
+    Proper (@Permutation ident ==> @Permutation equation ==> @eq (fresh_st (Op.type * clock * bool)) ==> @Basics.impl)
+           causal_inv.
+  Proof.
+    intros ? ? Hp1 ? ? Hp2 ? ? Heq Hcaus; subst.
+    unfold causal_inv in *.
+    destruct Hcaus as [Hndup1 [Hndup2 [ceqs [Hperm [Hcaus Hf]]]]].
+    repeat (split; try exists ceqs); auto.
+    - rewrite <- Hp1, <- Hp2; auto.
+    - rewrite <- Hp2; auto.
+    - rewrite <- Hp1; auto.
+  Qed.
+
+  Fact Is_causal_ck_causal_inv : forall inputs eqs id0,
+      NoDup (vars_defined eqs ++ inputs) ->
+      (exists ceqs, Permutation eqs ceqs /\
+               Is_causal_ck inputs ceqs) ->
+      causal_inv inputs eqs (init_st id0).
+  Proof.
+    intros * Hnd [ceqs [Hperm Hcaus]].
+    repeat (split; try exists ceqs); auto.
+    1,2: unfold st_inits; rewrite init_st_anns; simpl; constructor.
+  Qed.
+
+  Fact normalized_lexp_clockof : forall e,
+      normalized_lexp e ->
+      forall x, Exists (Is_free_in_clock x) (clockof e) -> Is_free_left_ck x e.
+  Proof.
+    intros * Hnormed ? Hex.
+    inv Hnormed; simpl in *; try destruct cl as [ck name]; apply Exists_singl in Hex; auto.
+    inv Hex.
+  Qed.
+
+  Fact untupled_equation_is_not_app_clockof : forall eq,
+      untupled_equation eq ->
+      Forall is_not_app (snd eq) ->
+      forall x, Exists (Is_free_in_clock x) (clocksof (snd eq)) -> Exists (Is_free_left_ck x) (snd eq).
+  Proof.
+    intros eq Hunt Hisnotapp ? Hex.
+    inv Hunt; simpl in *; auto.
+    1,2:apply Forall_singl in Hisnotapp; inv Hisnotapp.
+    constructor. inv H; simpl in *; auto.
+    1,2:destruct cl as [ck ?]; apply Exists_singl in Hex; auto.
+    rewrite app_nil_r in Hex.
+    eapply normalized_lexp_clockof; eauto.
+  Qed.
+
+  Fact insert_in {A : Type} : forall (l1 l2 l3 l4 : list A) (x : A),
+      l1 ++ l2 = l3 ++ x :: l4 ->
+      In x l1 \/ In x l2.
+  Proof.
+    intros * Heq.
+    assert (In x (l1++l2)).
+    { rewrite Heq, in_app_iff. right; left; auto. }
+    rewrite in_app_iff in H; auto.
+  Qed.
+
+  Fact NoDup_split {A : Type} : forall (l1 l2 l3 l4 : list A) (x : A),
+      NoDup (l1 ++ x :: l2) ->
+      l1 ++ x :: l2 = l3 ++ x :: l4 ->
+      l1 = l3 /\ l2 = l4.
+  Proof.
+    induction l1; intros * Hndup Heq; simpl in *.
+    - rewrite Heq in Hndup. destruct l3; simpl in *.
+      2:{ exfalso.
+          inv Heq. inv Hndup.
+          apply H1, in_or_app. right; left; auto. }
+      inv Heq; auto.
+    - inv Hndup.
+      destruct l3; simpl in *.
+      { exfalso. inv Heq. apply H1, in_or_app. right; left; auto. }
+      inv Heq.
+      eapply IHl1 in H2 as [? ?]; eauto.
+      split; f_equal; auto.
+  Qed.
+
+  Fact list_insert {A : Type} : forall (l1 l2 l3 l4 : list A) (x x' : A),
+      NoDup (l1 ++ l2) ->
+      l1 ++ l2 = l3 ++ x :: l4 ->
+      exists l5, exists l6, l1 ++ x' :: l2 = l5 ++ x :: l6 /\
+                  Permutation (l5 ++ l6) (x'::l3++l4) /\
+                  incl l3 l5.
+  Proof.
+    intros * Hndup Heq.
+    assert (Heq':=Heq).
+    eapply insert_in in Heq as [Hin|Hin];
+      eapply in_split in Hin as [l5 [l6 ?]]; subst.
+    - rewrite <- app_assoc, <- app_comm_cons in *.
+      eapply NoDup_split in Hndup as [? ?]; eauto; subst.
+      exists l3. exists (l6++x'::l2). repeat split; auto.
+      + rewrite Permutation_middle. apply Permutation_app_head.
+        rewrite <- Permutation_middle. apply perm_skip. reflexivity.
+      + reflexivity.
+    - rewrite app_assoc in *.
+      eapply NoDup_split in Hndup as [? ?]; eauto; subst.
+      exists (l1 ++ x'::l5). exists l4. repeat split; auto.
+      + rewrite <- app_assoc; auto.
+      + rewrite <- app_assoc, <- app_comm_cons, <- Permutation_middle.
+        apply perm_skip. rewrite <- app_assoc. reflexivity.
+      + apply incl_appr', incl_tl, incl_refl.
+  Qed.
+
+  Fact NoDup_vars_defined : forall G eqs,
+      Forall untupled_equation eqs ->
+      Forall (wl_equation G) eqs ->
+      NoDup (vars_defined eqs) ->
+      NoDup eqs.
+  Proof.
+    induction eqs; intros * Hunt Hwl Hnd. constructor.
+    simpl in Hnd.
+    inv Hunt. inv Hwl.
+    constructor.
+    - intro contra. destruct a as [xs es].
+      eapply untupled_equation_not_nil in H1; eauto; simpl in H1.
+      destruct xs; eauto.
+      eapply NoDup_app_In with (x:=i) in Hnd; simpl; eauto.
+      apply Hnd. unfold vars_defined. rewrite flat_map_concat_map.
+      eapply incl_concat_map; eauto; simpl; eauto.
+    - apply NoDup_app_r in Hnd; auto.
+  Qed.
+
+  Fact causal_inv_insert_early : forall G inputs eqs x ck e st st',
+      Forall untupled_equation eqs ->
+      Forall (wl_equation G) eqs ->
+      causal_inv inputs eqs st ->
+      clockof e = [ck] ->
+      ~In x (vars_defined eqs++inputs) ->
+      ~In ck (map snd (st_inits st)) ->
+      (forall x, Is_free_left_ck x e -> Is_free_in_clock x ck) ->
+      (forall x, Is_free_in_clock x ck -> In x (vars_defined eqs) \/ In x inputs) ->
+      st_inits st' = (x, ck)::st_inits st ->
+      causal_inv inputs (eqs++[([x], [e])]) st'.
+  Proof.
+    intros * Hunt Hwl Hcaus Hck Hnin1 Hnin2 Hfrees Hfreesck Hinits.
+    destruct Hcaus as [Hnd1 [Hnd2 [ceqs [Hperm [Hcaus Hf]]]]].
+    assert (forall x, Exists (Is_free_left_ck x) [e] -> In x (vars_defined ceqs) \/ In x inputs) as Hfrees'.
+    { intros ? Hex. rewrite <- Hperm. apply Exists_singl in Hex; auto. }
+    eapply causal_insert_early with (xs:=[x]) in Hfrees' as [eqs1 [eqs2 [? [Hcaus' Heqs']]]]; eauto; subst.
+    2:rewrite Hperm in Hnd1; auto.
+    repeat (split; try exists (eqs1++([x], [e])::eqs2)); auto.
+    - rewrite (Permutation_app_comm eqs _); simpl. constructor; auto.
+    - rewrite Hinits. simpl. constructor; auto.
+    - rewrite Permutation_app_comm, <- cons_is_app, <- Permutation_middle; auto.
+    - rewrite Hinits. constructor; auto.
+      + exists eqs1. exists eqs2. exists e.
+        rewrite Hperm in Hunt.
+        repeat split; auto.
+        solve_forall; simpl in *.
+        apply H0. intros ? Hex. apply Exists_singl in Hex; eauto.
+        eapply Hfrees in Hex. destruct H1 as [? [Heq [Hnapp Hck']]]; subst.
+        eapply untupled_equation_is_not_app_clockof in H2; simpl in *; eauto.
+        rewrite app_nil_r, Hck'; auto.
+      + eapply Forall_impl_In; [|eauto]. intros [? ?] ? [eqs3 [eqs4 [e' [? [? ?]]]]].
+        assert (c <> ck) as Hnck.
+        { intro contra; subst. apply Hnin2. simpl_In. exists (i, ck); auto. }
+        rewrite H0 in Hcaus.
+        assert (NoDup (eqs1++eqs2)) as Hndup'.
+        { rewrite <- Hperm. eapply NoDup_vars_defined; eauto.
+          apply NoDup_app_l in Hnd1; auto. }
+        specialize (list_insert _ _ _ _ _ ([x], [e]) Hndup' H0) as [eqs5 [eqs6 [Hins [Hperm' Hincl]]]].
+        exists eqs5. exists eqs6. exists e'. repeat split; auto. rewrite Hperm'.
+        constructor; auto.
+        * intros [? [? [? ?]]]; simpl in *. inv H3.
+          rewrite Hck in H5. inv H5. congruence.
+        * solve_forall.
+  Qed.
+
+  Fact init_var_for_clock_causal_inv : forall G inputs eqs ck x eqs' st st',
+      Forall untupled_equation eqs ->
+      Forall (wl_equation G) eqs ->
+      (forall x, Is_free_in_clock x ck -> In x (vars_defined eqs) \/ In x inputs) ->
+      weak_valid_after st (ps_from_list (vars_defined eqs++inputs)) ->
+      causal_inv inputs eqs st ->
+      init_var_for_clock ck st = (x, eqs', st') ->
+      causal_inv inputs (eqs++eqs') st'.
+  Proof.
+    intros * Hunt Hwl Hck Hvalid Hinv Hinit.
+    unfold init_var_for_clock in Hinit.
+    destruct (find _ _) eqn:Hfind.
+    - destruct p; inv Hinit; rewrite app_nil_r; auto.
+    - destruct (fresh_ident _ _) eqn:Hfresh. inv Hinit.
+      assert (Hfresh':=Hfresh). eapply fresh_ident_true_st_inits in Hfresh'.
+      eapply causal_inv_insert_early; simpl; eauto.
+      + eapply fresh_ident_weak_valid_nIn in Hfresh; eauto.
+        rewrite ps_from_list_In in Hfresh; auto.
+      + eapply st_inits_find_None; eauto.
+      + intros * Hfree. inv Hfree.
+        inv H0; apply Exists_singl in H; auto.
+        eapply add_whens_Is_free_left in H; eauto.
+  Qed.
+
+  Fact fresh_ident_false_causal_inv : forall inputs eqs a x st st',
+      causal_inv inputs eqs st ->
+      fresh_ident (a, false) st = (x, st') ->
+      causal_inv inputs eqs st'.
+  Proof.
+    intros * Hcaus Hfresh.
+    apply fresh_ident_false_st_inits in Hfresh.
+    unfold causal_inv in *. destruct Hcaus as [? [? [ceqs [? [? ?]]]]].
+    repeat (split; try exists ceqs); auto. 1,2:congruence.
+  Qed.
+
+  Fact fby_iteexp_causal_inv : forall G inputs eqs e0 e ty ck name e' eqs' st st',
+      Forall untupled_equation eqs ->
+      Forall (wl_equation G) eqs ->
+      normalized_lexp e0 ->
+      clockof e0 = [ck] ->
+      (forall x, Is_free_in_clock x ck -> In x (vars_defined eqs) \/ In x inputs) ->
+      weak_valid_after st (ps_from_list (vars_defined eqs++inputs)) ->
+      causal_inv inputs eqs st ->
+      fby_iteexp e0 e (ty, (ck, name)) st = (e', eqs', st') ->
+      exists eqs1, exists eqs2,
+          Permutation eqs' (eqs1++eqs2) /\
+          causal_inv inputs (eqs++eqs1) st' /\
+          Forall (fun eq => forall x, Exists (Is_free_left_ck x) (snd eq) -> Is_free_left_ck x e0) eqs2 /\
+          (forall x, Is_free_left_ck x e' ->
+                Is_free_left_ck x e0 \/ In (x, ck) (st_inits st') \/ In x (vars_defined eqs2)).
+  Proof.
+    intros * Hunt Hwl Hnormed Hck Hfreeck Hvalid [Hnd1 [Hnd2 [ceqs [Hperm [Hcaus Hf]]]]] Hfby.
+    unfold fby_iteexp in Hfby.
+    destruct (is_constant e0); repeat inv_bind; eauto.
+    - exists []. exists []. repeat rewrite app_nil_r. repeat (split; try exists ceqs); auto.
+      intros ? Hfree. inv Hfree; simpl. destruct H0.
+      + apply Exists_singl in H; auto.
+      + unfold clock_of_nclock, stripname in H. simpl in H. rewrite <- Hck in H.
+        eapply normalized_lexp_clockof in H; eauto.
+    - assert (H':=H). eapply init_var_for_clock_causal_inv in H'; eauto. 2:repeat (split; try exists ceqs); auto.
+      eapply fresh_ident_false_causal_inv in H'; eauto.
+      remember ([x2], _) as eq2.
+      exists x0; exists [eq2]; repeat (split; auto).
+      + rewrite Permutation_app_comm, <- cons_is_app; auto.
+      + constructor; auto.
+        intros ? Hex. subst; simpl in *.
+        apply Exists_singl in Hex. inv Hex. destruct H2 as [Hex|Hex].
+        * apply Exists_singl, add_whens_Is_free_left in Hex.
+          eapply normalized_lexp_clockof in Hnormed; eauto.
+          rewrite Hck; auto.
+        * eapply normalized_lexp_clockof in Hnormed; eauto.
+          rewrite Hck; auto.
+      + intros ? Hfree.
+        inv Hfree; simpl. destruct H2 as [Hfree|[Hfree|[Hfree|Hfree]]].
+        * inv Hfree. destruct H2 as [?|Hinit]; subst.
+          -- eapply init_var_for_clock_In_st_inits in H; eauto.
+             eapply fresh_ident_st_follows, st_follows_inits_incl in H0; auto.
+          -- eapply normalized_lexp_clockof in Hnormed; eauto.
+             rewrite Hck; auto.
+        * apply Exists_singl in Hfree; auto.
+        * apply Exists_singl in Hfree. inv Hfree. destruct H2 as [?|H2]; subst; auto.
+          eapply normalized_lexp_clockof in Hnormed; eauto.
+          rewrite Hck; auto.
+        * eapply normalized_lexp_clockof in Hnormed; eauto.
+          rewrite Hck; auto.
+  Qed.
+
+  Fact Permutation_split {A : Type} : forall (x : A) l l',
+      Permutation (x::l) l' ->
+      exists l1', exists l2', l' = l1' ++ x :: l2' /\ Permutation l (l1'++l2').
+  Proof.
+    intros * Hperm.
+    assert (Hin:=Hperm). eapply Permutation_in in Hin. 2:left; auto.
+    apply in_split in Hin as [l1' [l2' H]].
+    exists l1'. exists l2'. split; auto.
+    rewrite H, <- Permutation_middle in Hperm. apply Permutation_cons_inv in Hperm; auto.
+  Qed.
+
+  Fact Is_causal_ck_replace : forall inputs eq eqs1 eqs2 eqs',
+      Is_causal_ck inputs (eqs'++eqs2) ->
+      incl (vars_defined [eq]) (vars_defined eqs') ->
+      Is_causal_ck inputs (eqs1 ++ eq :: eqs2) ->
+      Is_causal_ck inputs (eqs1 ++ eqs' ++ eqs2).
+  Proof.
+    induction eqs1; intros * Hcaus1 Hincl Hcaus2; simpl in *; rewrite app_nil_r in *; auto.
+    inv Hcaus2. constructor; auto.
+    intros ? Hex. apply H2 in Hex.
+    repeat rewrite vars_defined_app, in_app_iff in *. simpl in *.
+    rewrite in_app_iff in Hex. destruct Hex as [[?|[?|?]]|?]; auto.
+  Qed.
+
+  Fact list_cut {A : Type} : forall (l1 l2 l3 l4 : list A) (x y : A),
+      l1 ++ x :: l2 = l3 ++ y :: l4 ->
+      NoDup (l1 ++ x :: l2) ->
+      In x l3 ->
+      In y l2.
+  Proof.
+    induction l1; intros * Heq Hnd Hin; simpl in *.
+    - assert (In y (l3 ++ y :: l4)) as Hin'.
+      { rewrite in_app_iff; simpl; auto. }
+      assert (x <> y) as Hneq.
+      { intro contra; subst. rewrite Heq in Hnd.
+        eapply NoDup_app_In in Hnd; eauto. apply Hnd; left; auto. }
+      rewrite <- Heq in Hin'. inv Hin'; auto. congruence.
+    - destruct l3; simpl in *; inv Heq; destruct Hin; subst.
+      + exfalso. inv Hnd. apply H2, in_or_app. right; left; auto.
+      + inv Hnd. eapply IHl1 in H1; eauto.
+  Qed.
+
+  Fact list_cut' {A : Type} : forall (l1 l2 l3 l4 : list A) (x y : A),
+      l1 ++ x :: l2 = l3 ++ y :: l4 ->
+      NoDup (l1 ++ x :: l2) ->
+      In x l4 ->
+      In y l1.
+  Proof.
+    intros l1 l2 l3. revert l1 l2.
+    induction l3; intros * Heq Hnd Hin; simpl in *.
+    - destruct l1; simpl in *.
+      + inv Heq. inv Hnd; auto.
+      + inv Heq; auto.
+    - destruct l1; simpl in *.
+      + inv Heq. inv Hnd.
+        apply H1, in_or_app. right. right. auto.
+      + inv Heq. inv Hnd. apply IHl3 in H1; auto.
+  Qed.
+
+  Fact NoDup_vars_defined_In : forall x e eqs1 eqs2,
+      NoDup (vars_defined(eqs1++eqs2)) ->
+      In x (vars_defined eqs1) ->
+      In ([x], [e]) (eqs1++eqs2) ->
+      In ([x], [e]) eqs1.
+  Proof.
+    intros * Hnd Hin1 Hin2.
+    apply in_app_iff in Hin2 as [Hin2|Hin2]; auto.
+    assert (In x (vars_defined eqs2)) as Hin3.
+    { unfold vars_defined. rewrite in_flat_map. exists ([x], [e]); split; simpl; auto. }
+    rewrite vars_defined_app in Hnd.
+    eapply NoDup_app_In in Hnd; eauto. congruence.
+  Qed.
+
+  Fact NoDup_split' {A} : forall (l1 l2 l3 l4 : list A) (x y : A),
+      NoDup (l1 ++ x :: l2) ->
+      x <> y ->
+      l1 ++ x :: l2 = l3 ++ y :: l4 ->
+      (exists l5, l3 = l1 ++ x :: l5 /\ l2 = l5 ++ y :: l4) \/
+      (exists l5, l4 = l5 ++ x :: l2 /\ l1 = l3 ++ y :: l5).
+  Proof.
+    induction l1; intros * Hnd Hneq Heq; simpl in *.
+    - destruct l3; simpl in *.
+      + inv Heq; congruence.
+      + inv Heq. left. exists l3; auto.
+    - inv Hnd.
+      destruct l3; simpl in *.
+      + inv Heq. right. exists l1; auto.
+      + inv Heq.
+        eapply IHl1 in H3 as [[l5 [? ?]]|[l5 [? ?]]]; subst; eauto.
+  Qed.
+
+  Fact causal_replace : forall G inputs x e ck eqs eqs' st,
+      Forall untupled_equation (([x], [e])::eqs) ->
+      Forall (wl_equation G) (([x], [e])::eqs) ->
+      is_not_app e ->
+      clockof e = [ck] ->
+      Forall (fun eq => clocksof (snd eq) = [ck]) eqs' ->
+      (forall inputs, Is_causal_ck inputs [([x], [e])] ->
+                 Is_causal_ck (inputs++map fst (filter (fun '(_, ck') => ck' ==b ck) (st_inits st))) eqs') ->
+      In x (vars_defined eqs') ->
+      ~In x (map fst (st_inits st)) ->
+      NoDup (vars_defined (eqs' ++ eqs) ++ inputs) ->
+      causal_inv inputs (([x], [e])::eqs) st ->
+      causal_inv inputs (eqs'++eqs) st.
+  Proof.
+    intros * Hunt Hwl Hnapp Hck1 Hck2 Hcaus1 Hin Hnin Hnd [Hnd1 [Hnd2 [ceqs [Hperm [Hcaus2 Hf]]]]].
+    repeat split; auto.
+    apply Permutation_split in Hperm as [ceqs1 [ceqs2 [Heq Hperm']]]; subst.
+    assert (NoDup (ceqs1 ++ ([x], [e]) :: ceqs2)) as Hnd'.
+    { eapply NoDup_vars_defined.
+        1,2,3: rewrite <- Permutation_middle, <- Hperm'; eauto.
+        apply NoDup_app_l in Hnd1; auto. }
+    (* since the eqs' only use the st_init based on ck, they respond to the property in Hf,
+       which means the relevant st_inits are included into the vars defined by the ceqs2.
+       This will be useful twice *)
+    assert (Forall (fun '(x, ck') => ck' = ck -> In x (vars_defined ceqs2)) (st_inits st)) as Hinits.
+    { eapply Forall_impl_In; [|eauto]. intros; destruct_conjs; clear Hf.
+      intros Heq. simpl in Hck1; subst.
+      destruct H0 as [eqs1 [eqs2 [? [Heq [Hck' Hf]]]]].
+      assert (x <> i) as Hneq.
+      { intro contra; subst. apply Hnin. simpl_In. exists (i, ck); auto. }
+      assert (In ([x], [e]) (eqs1++eqs2)) as Hin'.
+      { symmetry in Heq. apply insert_in in Heq; simpl in Heq.
+        rewrite in_app_iff. destruct Heq as [Heq|[Heq|Heq]]; auto.
+        inv Heq; congruence. }
+      eapply Forall_forall in Hin'; eauto; simpl in Hin'.
+      eapply list_cut in Heq; auto.
+      * unfold vars_defined. rewrite flat_map_concat_map.
+        apply in_concat. exists [i]; split. left; auto.
+        simpl_In. exists ([i], [x0]); auto.
+      * eapply Hin'. exists e; auto.
+    }
+    exists (ceqs1++eqs'++ceqs2). repeat split; auto.
+    - rewrite Hperm', Permutation_swap; auto.
+    - eapply Is_causal_ck_replace; eauto.
+      2:{ simpl. intros ? Hin'. apply In_singleton in Hin'; subst; auto. }
+      apply Is_causal_ck_appr in Hcaus2.
+      eapply Is_causal_ck_app.
+      + inv Hcaus2; auto.
+      + rewrite cons_is_app in Hcaus2.
+        eapply Is_causal_ck_appl, Hcaus1 in Hcaus2.
+        eapply Is_causal_ck_incl; eauto.
+        apply incl_app; [apply incl_refl|].
+        apply incl_appr.
+        intros ? Hin'. repeat simpl_In.
+        rewrite filter_In in H0; destruct H0 as [Hin' Hck']. rewrite clock_eqb_eq in Hck'; subst.
+        eapply Forall_forall in Hin'; eauto. simpl in *; auto.
+    - solve_forall.
+      destruct H1 as [eqs1 [eqs2 [? [Heq [Hck' Hf]]]]].
+      (* if c = ck, then i is in ceqs2, so ([x], [e]) is in eqs1 OK ?
+         if c <> ck no constraint *)
+      destruct (equiv_decb c ck) eqn:Heqck.
+      + rewrite clock_eqb_eq in Heqck; subst. specialize (H0 eq_refl).
+        assert (In ([i], [x0]) (([x], [e])::eqs)) as Hin'.
+        { rewrite Hperm', Permutation_middle. setoid_rewrite Heq.
+          apply in_or_app. right. left. auto. }
+        assert(Heq':=Heq). symmetry in Heq. eapply list_cut' in Heq.
+        2:(setoid_rewrite Heq; auto).
+        2:{ eapply NoDup_vars_defined_In with (eqs2:=(([x], [e])::ceqs1)); eauto.
+            + rewrite Hperm', app_comm_cons in Hnd1. apply NoDup_app_l in Hnd1.
+              rewrite vars_defined_app in *; simpl. rewrite <- Permutation_middle, Permutation_app_comm; auto.
+            + rewrite <- Permutation_middle, Permutation_app_comm, <- Hperm'; auto. }
+        apply in_split in Heq as [eqs3 [eqs4 Heq]]; subst.
+        rewrite <- app_assoc, <- app_comm_cons in Heq'.
+        apply NoDup_split in Heq' as [Heq1 Heq2]; auto; simpl in *; subst.
+        exists (eqs3++eqs'++eqs4). exists eqs2. exists x0.
+        repeat split; auto.
+        * repeat rewrite <- app_assoc; auto.
+        * simpl in Hf. repeat rewrite <- app_assoc in *.
+          assert (Forall (fun equ => not (equ = ([x], [e]))) (eqs3 ++ eqs4 ++ eqs2)) as Hneq.
+          { rewrite <- Permutation_middle in Hnd'. inv Hnd'.
+            eapply Forall_forall. intros ? Hin'' contra; subst.
+            apply H3. repeat rewrite in_app_iff in *. destruct Hin'' as [?|[?|?]]; auto.
+            right. right. right. auto. }
+          clear - Hf Hneq.
+          repeat rewrite Forall_app in *. destruct Hf as [Hf1 [Hf2 Hf3]]. inv Hf2.
+          destruct Hneq as [Hneq1 [Hneq2 Hneq3]].
+          repeat split.
+          1,3,4:solve_forall; repeat rewrite in_app_iff in *; simpl in *; auto.
+          -- eapply H3 in H2. destruct H2 as [?|[?|?]]; auto. congruence.
+          -- eapply Forall_forall. intros. repeat rewrite in_app_iff. right. left. auto.
+      + rewrite clock_eqb_neq in Heqck. clear H0.
+        assert (([x], [e]) <> ([i], [x0])) as Hneq.
+        { intro contra. inv contra. rewrite Hck1 in Hck'. inv Hck'. congruence. }
+        symmetry in Heq. eapply NoDup_split' in Heq as [[eqs5 [? ?]]|[eqs5 [? ?]]]; subst; eauto.
+        3:setoid_rewrite Heq; auto.
+        1: (exists eqs1; exists (eqs5++eqs'++ceqs2); exists x0). 2: (exists (ceqs1++eqs'++eqs5); exists eqs2; exists x0).
+        1,2:repeat split; repeat rewrite <- app_assoc; auto.
+        1,2:repeat rewrite Forall_app in *.
+        * destruct Hf as [Hf1 [Hf2 Hf3]]; inv Hf3.
+          repeat split; auto.
+          solve_forall; simpl in *.
+          destruct H4 as [? [? [? Hck'']]]; subst. simpl in H1; rewrite app_nil_r in H1.
+          rewrite H1 in Hck''. inv Hck''. congruence.
+        * assert (Forall (fun equ => not (equ = ([x], [e]))) (ceqs1 ++ eqs2 ++ eqs5)) as Hneq'.
+          { rewrite <- (Permutation_middle ceqs1) in Hnd'. inv Hnd'.
+            eapply Forall_forall. intros ? Hin'' contra; subst.
+            apply H2. repeat rewrite in_app_iff in *. destruct Hin'' as [?|[?|?]]; auto.
+            right. right. right. auto. }
+          clear - Hf Hck2 Heqck Hneq'.
+          destruct Hf as [[Hf1 Hf2] Hf3].
+          repeat rewrite Forall_app in Hneq'. destruct Hneq' as [? [? ?]].
+          repeat split.
+          1,3,4:solve_forall; repeat rewrite in_app_iff in *; simpl in *; auto.
+          -- eapply H3 in H2. destruct H2 as [?|[?|?]]; auto. congruence.
+          -- solve_forall. destruct H2 as [? [? [? Hck'']]]; simpl in *; subst.
+             simpl in H0; rewrite app_nil_r in H0. rewrite H0 in Hck''. inv Hck''. congruence.
+  Qed.
+
+  Fact fby_equation_causal : forall G vars to_cut inputs eq eqs eqs' st st',
+      Forall untupled_equation (eq::eqs) ->
+      Forall (wl_equation G) (eq::eqs) ->
+      wc_equation G vars eq ->
+      weak_valid_after st (ps_from_list (vars_defined (eq::eqs)++inputs)) ->
+      Forall (fun id => ~In id (map fst (st_inits st))) (vars_defined [eq]) ->
+      causal_inv inputs (eq::eqs) st ->
+      fby_equation to_cut eq st = (eqs', st') ->
+      causal_inv inputs (eqs++eqs') st'.
+  Proof.
+    intros * Hunt Hwl Hwc Hvalid Hnin Hinv Hfby.
+    inv_fby_equation Hfby to_cut eq.
+    2: { rewrite cons_is_app, Permutation_app_comm in Hinv; auto. }
+    destruct x2 as [ty [ck name]]; repeat inv_bind.
+    assert (normalized_lexp x0) as Hnormed.
+    { inv Hunt. inv H3; auto. inv H2. inv H1. }
+    assert (clockof x0 = [ck]) as Hck.
+    { destruct Hwc as [Hwc _]. apply Forall_singl in Hwc. inv Hwc; simpl in *.
+      rewrite Forall2_eq, app_nil_r in H6; auto. }
+    assert (weak_valid_after st (ps_from_list (vars_defined eqs++inputs))) as Hvalid2.
+    { eapply weak_valid_after_Subset; eauto. rewrite <- add_ps_from_list_cons.
+      apply PSP.subset_add_2. reflexivity. }
+    assert (Hnd':=H). eapply fby_iteexp_NoDup in Hnd'; eauto.
+    2:{ destruct Hinv as [Hnd _]; simpl in Hnd. inv Hnd; auto. }
+    assert (Hfby:=H). eapply fby_iteexp_causal_inv in H as [eqs1 [eqs2 [Hperm [Hcaus [Heqs2 He']]]]]; eauto; auto.
+    - destruct (PS.mem _ _); repeat inv_bind.
+      + rewrite Hperm, Permutation_app_comm, (Permutation_app_comm eqs1); simpl.
+        rewrite <- app_assoc, (Permutation_app_comm eqs1).
+        eapply causal_replace with (eqs':=([x], [Evar x5 (ty, (ck, name))])::([x5], [x2])::eqs2) in Hcaus; simpl in *; eauto.
+        2,3:rewrite app_comm_cons, Forall_app; split; eauto.
+        * eapply fresh_ident_false_causal_inv; eauto.
+        * eapply fby_iteexp_untupled_eq with (a:=(ty, (ck, name))) in Hfby; eauto.
+          rewrite Hperm, Forall_app in Hfby; destruct Hfby; auto.
+          inv Hunt. inv H2; auto. inv H1;inv H0.
+        * inv Hwl. inv H2.
+          apply Forall_singl in H0. inv H0; simpl in *.
+          apply Forall_singl in H6. apply Forall_singl in H8.
+          rewrite app_nil_r, length_annot_numstreams in *.
+          eapply fby_iteexp_wl_eq with (a:=(ty, (ck, name))) in Hfby; eauto.
+          rewrite Hperm, Forall_app in Hfby. destruct Hfby; auto.
+        * repeat constructor; simpl.
+          -- rewrite app_nil_r.
+             eapply fby_iteexp_annot with (ann0:=(ty, (ck, name))) in Hfby.
+             rewrite clockof_annot, Hfby; auto.
+          -- eapply fby_iteexp_clocksof in Hfby; eauto.
+             rewrite Hperm, Forall_app in Hfby. destruct Hfby; auto.
+        * intros ? Hcaus'.
+          constructor; [constructor|]; simpl; auto.
+          -- inv Hcaus'. clear H2.
+             eapply Is_causal_ck_Forall'.
+             solve_forall; simpl in *.
+             eapply H1 in H2.
+             rewrite in_app_iff.
+             assert (False \/ In x6 inputs0) as [Hf|?]; eauto. 2:inv Hf.
+             eapply H3; auto.
+          -- intros ? Hex. apply Exists_singl in Hex. apply He' in Hex.
+             rewrite in_app_iff. destruct Hex as [Hex|[?|?]]; auto.
+             ++ inv Hcaus'. clear H2; simpl in *.
+               assert (False \/ In x6 inputs0) as [Hf|?]; eauto. 2:inv Hf.
+               eapply H3; auto.
+             ++ right. right. simpl_In.
+                exists (x6, ck); split; auto. apply filter_In; split; auto.
+                apply equiv_decb_refl.
+          -- intros ? Hex. apply Exists_singl in Hex. inv Hex. destruct H1 as [?|Hex]; auto.
+             inv Hcaus'; clear H2. specialize (H3 x6); simpl in H3.
+             rewrite in_app_iff.
+             assert (False \/ In x6 inputs0) as [Hf|?]; auto. 2:inv Hf.
+             apply H3. constructor. constructor. right; simpl. constructor; auto.
+        * clear - Hnin Hvalid Hfby.
+          eapply fby_iteexp_weak_valid_nIn_st_inits with (a:=(ty, (ck, name))) in Hfby; eauto. 2:inv Hnin; auto.
+          rewrite <- add_ps_from_list_cons. apply PSF.add_1; auto.
+        * constructor; [|constructor].
+          -- intro contra.
+             clear Hvalid2. assert (Hfby':=Hfby). eapply fby_iteexp_weak_valid_nIn with (a:=(ty, (ck, name))) in Hfby; eauto.
+             2:rewrite <- add_ps_from_list_cons; apply PSF.add_1; reflexivity.
+             rewrite Hperm in Hfby.
+             destruct Hcaus as [Hcaus _]. simpl in *; inv Hcaus.
+             repeat rewrite vars_defined_app in *. repeat rewrite in_app_iff in *.
+             destruct contra as [?|[[?|[?|?]]|?]]; subst; auto.
+             eapply fresh_ident_weak_valid_nIn in H; eauto.
+             2:eapply fby_iteexp_weak_valid with (eqs:=([x], [Efby [x0] [x1] [(ty, (ck, name))]])::eqs) in Hfby'; simpl in *; eauto.
+             eapply H. rewrite ps_from_list_In. left; auto.
+          -- eapply fby_iteexp_weak_valid in Hfby; eauto.
+             eapply fresh_ident_weak_valid_nIn in H; eauto.
+             rewrite ps_from_list_In, Hperm in H.
+             rewrite (Permutation_app_swap eqs1), app_assoc, (Permutation_app_comm _ eqs2), <- app_assoc in H; auto.
+          -- rewrite Permutation_app_comm in Hperm. rewrite Hperm, Permutation_swap in Hnd'; auto.
+      + rewrite Hperm, Permutation_app_comm, (Permutation_app_comm eqs1); simpl.
+        rewrite <- app_assoc, (Permutation_app_comm eqs1).
+        eapply causal_replace with (eqs':=([x], [x2])::eqs2) in Hcaus; simpl in *; eauto.
+        1,2:rewrite app_comm_cons, Forall_app; split; eauto.
+        * eapply fby_iteexp_untupled_eq with (a:=(ty, (ck, name))) in Hfby; eauto.
+          rewrite Hperm, Forall_app in Hfby; destruct Hfby; auto.
+          inv Hunt. inv H1; auto. inv H0;inv H.
+        * inv Hwl. inv H1.
+          apply Forall_singl in H. inv H; simpl in *.
+          apply Forall_singl in H5. apply Forall_singl in H7.
+          rewrite app_nil_r, length_annot_numstreams in *.
+          eapply fby_iteexp_wl_eq with (a:=(ty, (ck, name))) in Hfby; eauto.
+          rewrite Hperm, Forall_app in Hfby. destruct Hfby; auto.
+        * constructor; simpl.
+          -- rewrite app_nil_r.
+             eapply fby_iteexp_annot with (ann0:=(ty, (ck, name))) in Hfby.
+             rewrite clockof_annot, Hfby; auto.
+          -- eapply fby_iteexp_clocksof in Hfby; eauto.
+             rewrite Hperm, Forall_app in Hfby. destruct Hfby; auto.
+        * intros ? Hcaus'.
+          constructor; auto.
+          -- inv Hcaus'. clear H1.
+             eapply Is_causal_ck_Forall'.
+             solve_forall; simpl in *.
+             eapply H0 in H1.
+             assert (False \/ In x4 inputs0) as [Hf|?]; eauto. 2:inv Hf.
+             eapply H2; auto. rewrite in_app_iff; auto.
+          -- intros ? Hex. apply Exists_singl in Hex. apply He' in Hex.
+             rewrite in_app_iff. destruct Hex as [Hex|[?|?]]; auto.
+             ++ inv Hcaus'. clear H1; simpl in *.
+               assert (False \/ In x4 inputs0) as [Hf|?]; eauto. 2:inv Hf.
+               eapply H2; auto.
+             ++ right. right. simpl_In.
+                exists (x4, ck); split; auto. apply filter_In; split; auto.
+                apply equiv_decb_refl.
+        * clear - Hnin Hvalid Hfby.
+          eapply fby_iteexp_weak_valid_nIn_st_inits with (a:=(ty, (ck, name))) in Hfby; eauto. 2:inv Hnin; auto.
+          rewrite <- add_ps_from_list_cons. apply PSF.add_1; auto.
+        * simpl. constructor; auto.
+          -- intro contra.
+             clear Hvalid2.
+             eapply fby_iteexp_weak_valid_nIn with (id:=x) (a:=(ty, (ck, name))) in Hfby; [| |eauto].
+             2:rewrite <- add_ps_from_list_cons. 2:apply PSF.add_1; auto.
+             rewrite Hperm in Hfby.
+             destruct Hcaus as [Hcaus _]. simpl in Hcaus; inv Hcaus.
+             repeat rewrite vars_defined_app in *. repeat rewrite in_app_iff in *.
+             destruct contra as [[?|[?|?]]|?]; auto.
+          -- rewrite Permutation_app_comm in Hperm. rewrite Hperm, Permutation_swap in Hnd'; auto.
+    - clear - Hinv Hck Hnormed. intros ? Hfree.
+      eapply normalized_lexp_clockof in Hnormed. 2:rewrite Hck; eauto.
+      destruct Hinv as [_ [_ [ceqs [Hperm [Hcaus _]]]]]. rewrite Hperm.
+      eapply Permutation_in in Hperm. 2:left; eauto.
+      eapply Is_causal_ck_Forall, Forall_forall in Hcaus; eauto.
+      eapply Hcaus; simpl; auto.
+  Qed.
+
+  Fact fby_equations_causal' : forall G vars to_cut inputs eqs ceqs eqs' st st',
+      Forall untupled_equation (ceqs++eqs) ->
+      Forall (wl_equation G) (ceqs++eqs) ->
+      Forall (wc_equation G vars) eqs ->
+      weak_valid_after st (ps_from_list (vars_defined (ceqs++eqs)++inputs)) ->
+      Forall (fun id => ~In id (map fst (st_inits st))) (vars_defined eqs) ->
+      causal_inv inputs (ceqs++eqs) st ->
+      fby_equations to_cut eqs st = (eqs', st') ->
+      causal_inv inputs (ceqs++eqs') st'.
+  Proof.
+    induction eqs; intros * Hunt Hwl Hwc Hvalid Hnin Hinv Hfby;
+      unfold fby_equations in Hfby; simpl in *; repeat inv_bind; simpl; auto.
+    inv Hwc.
+    rewrite <- Permutation_middle in Hinv.
+    assert (Hvalid':=H). eapply fby_equation_weak_valid in Hvalid'.
+    2:{ rewrite (Permutation_app_comm ceqs), <- app_comm_cons in Hvalid; eauto. }
+    apply Forall_app in Hnin as [Hnin1 Hnin2].
+    eapply fby_equation_causal in H as Hcaus'. 4,7:eauto.
+    2,3:rewrite Permutation_middle; eauto.
+    3:simpl; rewrite app_nil_r; auto. 2:rewrite Permutation_middle; auto.
+    rewrite <- app_assoc, (Permutation_app_comm eqs), app_assoc in Hcaus'.
+    eapply IHeqs in Hcaus'; eauto.
+    - rewrite <- app_assoc in Hcaus'; eauto.
+    - apply Forall_app in Hunt as [Hunt1 Hunt2]. inv Hunt2.
+      repeat rewrite Forall_app. repeat split; auto.
+      eapply fby_equation_untupled_eq; eauto.
+    - apply Forall_app in Hwl as [Hwl1 Hwl2]. inv Hwl2.
+      repeat rewrite Forall_app. repeat split; auto.
+      eapply fby_equation_wl; eauto.
+    - rewrite <- app_assoc in *. rewrite (Permutation_app_comm x0), app_assoc, (Permutation_app_comm ceqs), <- app_assoc; auto.
+    - solve_forall. eapply fby_equation_weak_valid_nIn_st_inits in H; eauto.
+      rewrite ps_from_list_In, vars_defined_app; simpl.
+      repeat rewrite in_app_iff; auto.
+    - unfold fby_equations; repeat inv_bind; repeat eexists; eauto; inv_bind; auto.
+  Qed.
+
+  Corollary fby_equations_causal : forall G vars to_cut inputs eqs eqs' st st',
+      Forall untupled_equation eqs ->
+      Forall (wc_equation G vars) eqs ->
+      weak_valid_after st (ps_from_list (vars_defined eqs++inputs)) ->
+      Forall (fun id => ~In id (map fst (st_inits st))) (vars_defined eqs) ->
+      causal_inv inputs eqs st ->
+      fby_equations to_cut eqs st = (eqs', st') ->
+      causal_inv inputs eqs' st'.
+  Proof.
+    intros * Hunt Hwl Hvalid Hnin Hcaus Hfby.
+    eapply fby_equations_causal' with (ceqs:=[]) in Hfby; simpl; eauto.
+    solve_forall.
+  Qed.
+
+  Lemma normfby_node_causal : forall G n to_cut Hunt,
+      wc_global G ->
+      wc_node G n ->
+      node_causal n ->
+      node_causal (normfby_node to_cut n Hunt).
+  Proof.
+    intros * HwcG Hwc Hcaus.
+    unfold node_causal in *; simpl.
+    remember (fby_equations _ _ _) as res. symmetry in Heqres. destruct res as [eqs' st'].
+    eapply fby_equations_causal with (inputs:=map fst (n_in n)) in Heqres; eauto.
+    - destruct Heqres as [? [? [ceqs [Hperm [Hcaus' _]]]]].
+      exists ceqs; simpl; split; auto.
+      apply Is_causal_ck_Is_causal; auto.
+    - destruct Hwc as [_ [_ [_ Hwc]]]; eauto.
+    - eapply st_valid_weak_valid, init_st_valid.
+      rewrite PS_For_all_Forall', n_defd.
+      eapply Forall_incl. 1:eapply first_unused_ident_gt; reflexivity.
+      rewrite <- map_app, Permutation_app_comm.
+      apply incl_tl, incl_tl, incl_map, incl_appr', incl_appr', incl_appl, incl_refl.
+    - eapply Forall_forall; intros ? _.
+      unfold st_inits. rewrite init_st_anns. simpl; auto.
+    - apply Is_causal_ck_causal_inv; auto.
+      + specialize (n_nodup n) as Hnd.
+        rewrite n_defd, <- map_app, <- fst_NoDupMembers, Permutation_app_comm.
+        repeat rewrite app_assoc in *. apply NoDupMembers_app_l in Hnd; auto.
+      + destruct Hcaus as [ceqs [Hperm Hcaus]].
+        exists ceqs. split; auto.
+        rewrite <- map_fst_idck.
+        eapply Is_causal_Is_causal_ck; eauto.
+        5:(destruct Hwc as [_ [_ [_ Hwc]]]; rewrite Hperm in Hwc; eauto).
+        * unfold idck.
+          apply incl_map, incl_appl, incl_refl.
+        * rewrite NoDupMembers_idck.
+          specialize (n_nodup n) as Hnd.
+          repeat rewrite app_assoc in *. apply NoDupMembers_app_l in Hnd; auto.
+        * unfold untupled_node in Hunt. rewrite <- Hperm; auto.
+        * destruct Hwc; auto.
+        * rewrite map_fst_idck; auto.
+  Qed.
+
+  Lemma normfby_global_causal : forall G Hunt,
+      wc_global G ->
+      Forall node_causal G ->
+      Forall node_causal (normfby_global G Hunt).
+  Proof.
+    induction G; intros * Hwc Hcaus; auto.
+    inv Hwc. inv Hcaus.
+    constructor; eauto.
+    eapply normfby_node_causal; eauto.
+  Qed.
+
+End NCAUSALITY.
+
+Module NCausalityFun
+       (Ids : IDS)
+       (Op : OPERATORS)
+       (OpAux : OPERATORS_AUX Op)
+       (Syn : LSYNTAX Ids Op)
+       (Clo : LCLOCKING Ids Op Syn)
+       (Cau : LCAUSALITY Ids Op Syn)
+       (Norm : NORMALIZATION Ids Op OpAux Syn)
+       <: NCAUSALITY Ids Op OpAux Syn Clo Cau Norm.
+  Include NCAUSALITY Ids Op OpAux Syn Clo Cau Norm.
+End NCausalityFun.
